Overhaul of the De Morgan proof

DeMorgan.thy
@@ -8,165 +8,7 @@ type_synonym dalphabet = "dm_conn alphabet"
 type_synonym dfrege = "(string, dm_conn) frege"
 type_synonym dproof = "(string, dm_conn) frege_proof"
 
-function rule_to_taut :: "drule \<Rightarrow> dformula" where
-  "rule_to_taut \<lparr>prems = [], concl = c\<rparr> = c" |
-  "rule_to_taut \<lparr>prems = f # fs, concl = c\<rparr> = 
-    Conn Or [Conn Not [f], rule_to_taut \<lparr>prems = fs, concl = c\<rparr>]"
-  by pat_completeness auto
-termination
-  by (relation "measure (\<lambda>r. length (prems r))") auto
-
-definition modus_ponens :: drule where
-  "modus_ponens = \<lparr> 
-    prems = [
-      Atom ''P'', 
-      Conn Or [Conn Not [Atom ''P''], Atom ''Q'']
-    ], 
-    concl = Atom ''Q'' 
-  \<rparr>"
-
-
-locale de_morgan_frege =
-  fixes F :: dfrege
-  assumes conns_def: "conns (alphabet F) = {Top, Bot, Not, Or, And}"
-  and arity_def: "arity (alphabet F) = (\<lambda>c. case c of Top \<Rightarrow> 0 | Bot \<Rightarrow> 0 | Not \<Rightarrow> 1 | Or \<Rightarrow> 2 | And \<Rightarrow> 2)"
-  and conn_evals_def: "conn_evals (alphabet F) = (\<lambda> c. case c of
-    Top \<Rightarrow> (\<lambda>_. True)                \<comment> \<open>nullary: ignores input list\<close>
-  | Bot \<Rightarrow> (\<lambda>_. False)               \<comment> \<open>nullary\<close>
-  | Not \<Rightarrow> (\<lambda>args. case args of [x] \<Rightarrow> \<not> x | _ \<Rightarrow> undefined)
-  | Or  \<Rightarrow> (\<lambda>args. case args of [x, y] \<Rightarrow> x \<or> y | _ \<Rightarrow> undefined)
-  | And \<Rightarrow> (\<lambda>args. case args of [x, y] \<Rightarrow> x \<and> y | _ \<Rightarrow> undefined))"
-  and "frege_system F"
-begin
-
-abbreviation a where "a \<equiv> alphabet F"
-
-(*
-1. Either one of the premises is false, then the formula is true (\<not>f \<or> ...)
-2. Or all of the premises are true and by soundness the conclusion is also true (\<not>f \<or> ... \<or> q)
-*)
-
-lemma taut_unfold: "prems r = p # ps \<longrightarrow> eval a val (rule_to_taut r) = ((\<not> eval a val p) \<or> 
-                         eval a val (rule_to_taut \<lparr>prems = ps, concl = concl r\<rparr>))"
-proof
-  assume pr: "prems r = p # ps"
-
-  have r_eq: "r = \<lparr>prems = p # ps, concl = concl r\<rparr>"
-    using pr by (cases r) auto
-
-  show "eval a val (rule_to_taut r) =
-   ((\<not> eval a val p) \<or> eval a val (rule_to_taut \<lparr>prems = ps, concl = concl r\<rparr>))"
-  proof -
-    have "eval a val (rule_to_taut r) = eval a val (rule_to_taut \<lparr>prems = p # ps, concl = concl r\<rparr>)"
-      using r_eq by simp
-    also have "... = eval a val (Conn Or [Conn Not [p],
-                            rule_to_taut \<lparr>prems = ps, concl = concl r\<rparr>])"
-      by auto
-    also have "... = (eval a val (Conn Not [p]) \<or> 
-                      eval a val (rule_to_taut \<lparr>prems = ps, concl = concl r\<rparr>))"
-      using de_morgan_frege_axioms de_morgan_frege_def by auto
-    also have "... = ((\<not> eval a val p) \<or> 
-                         eval a val (rule_to_taut \<lparr>prems = ps, concl = concl r\<rparr>))"
-      using de_morgan_frege_axioms de_morgan_frege_def by auto
-    finally show ?thesis .
-  qed
-qed
-
-lemma premise_false:
-  fixes val :: "string \<Rightarrow> bool"
-  and r :: drule
-assumes "\<exists> f \<in> set (prems r). \<not> eval a val f"
-  and "prems r \<noteq> []"
-shows "eval a val (rule_to_taut r)"
-  using assms
-proof (induction "prems r" arbitrary: r)
-  case Nil
-  thus ?case by auto
-next
-  case (Cons p ps)
-  show ?case
-  proof (cases "\<not> eval a val p")
-    case True
-    show ?thesis using Cons True taut_unfold[of r p ps val] by auto
-  next
-    case False
-    have "\<exists> g \<in> set (p # ps). \<not> eval a val g" using Cons assms(1) by auto
-    hence g: "\<exists> g \<in> set ps. \<not> eval a val g" using False by auto
-    hence "ps \<noteq> []" by auto
-    hence "eval a val (rule_to_taut \<lparr>prems = ps, concl = concl r\<rparr>)" using g Cons by auto
-    thus ?thesis using taut_unfold[of r p ps val] Cons by auto
-  qed
-qed
-
-lemma premises_true:
-  fixes val :: "string \<Rightarrow> bool"
-  and r :: drule
-assumes "eval a val (concl r)"
-shows "eval a val (rule_to_taut r)"
-  using assms
-proof (induction "prems r" arbitrary: r)
-  case Nil
-  have "r = \<lparr> prems = [], concl = concl r\<rparr>" using Nil by simp
-  hence "eval a val (rule_to_taut r) = eval a val (rule_to_taut \<lparr>prems = [], concl = concl r\<rparr>)" 
-    by simp
-  also have  "... = eval a val (concl r)" by simp
-  finally have "eval a val (rule_to_taut r) = eval a val (concl r)" by simp
-  thus ?case using Nil.prems by simp
-next
-  case (Cons p ps)
-  have eq: "eval a val (rule_to_taut r) = ((\<not> eval a val p) \<or> 
-                         eval a val (rule_to_taut \<lparr>prems = ps, concl = concl r\<rparr>))"
-    using Cons taut_unfold[of r p ps val] by simp
-  have "eval a val (rule_to_taut \<lparr>prems = ps, concl = concl r\<rparr>)" using Cons by simp
-  thus ?case using eq by simp
-qed
-
-
-lemma sound_rule_gives_tautology:
-  assumes "r \<in> rules F"
-shows "\<forall> val. eval a val (rule_to_taut r)"
-proof
-  fix val
-  show "eval a val (rule_to_taut r)"
-  proof (cases "\<exists> f \<in> set (prems r). \<not> eval a val f")
-    case True
-    have "prems r \<noteq> []" using True by auto
-    thus ?thesis using True premise_false by simp
-  next
-    case False
-    have all_prems_true: "\<forall> f \<in> set (prems r). eval a val f" using False by simp
-    have "sound_rule F r" 
-      using assms de_morgan_frege_def de_morgan_frege_axioms frege_system.sound by auto
-    hence "eval a val (concl r)" using all_prems_true sound_rule_def[of F r] by simp 
-    thus ?thesis using premises_true by simp
-  qed
-qed
-
-end
-
-lemma proof_exists_for_rule:
-  assumes "frege_system F \<and> de_morgan_frege F"
-      and "frege_system F' \<and> de_morgan_frege F'"
-      and "rule \<in> rules F"
-    shows "\<exists> pr. valid_proof F' pr \<and> assumptions pr = set (prems rule) \<and> thesis pr = concl rule"
-proof -
-  have "alphabet F = alphabet F'"
-    using assms(1,2) de_morgan_frege_def by fastforce
-  hence val_sat: "\<forall> val. (\<forall> f \<in> set (prems rule). eval (alphabet F') val f) 
-                \<longrightarrow> eval (alphabet F') val (concl rule)"
-    using assms(1,3) frege_system.sound sound_rule_def
-    by metis 
-  have "(\<forall> val. (\<forall> f \<in> set (prems rule). eval (alphabet F') val f) \<longrightarrow> 
-                 eval (alphabet F') val (concl rule)) 
-                          \<longrightarrow> (\<exists> pr. valid_proof F' pr
-                                   \<and> assumptions pr = set (prems rule) 
-                                   \<and> thesis pr = concl rule)"
-    using assms(2) frege_system_def by auto
-  thus ?thesis using val_sat
-    by force
-qed
-
-(* Predicate for a step being derived with a rule, a substitution, and as i-th step of a proof. *)
+(* -- General lemmas that might be useful for the main proof as well -- *)
 definition derived_with :: "nat \<Rightarrow> dproof \<Rightarrow> drule \<Rightarrow> (string \<Rightarrow> dformula) \<Rightarrow> bool" where
   "derived_with i pr r s \<longleftrightarrow> (let sub_r = sub_rule s r in
                        i < length (steps pr) \<and> (concl sub_r) = steps pr ! i \<and>
@@ -216,7 +58,42 @@ proof -
   qed
 qed
 
-context de_morgan_frege begin
+lemma var_set_rule_finite:
+  shows "finite (var_set_rule r)"
+proof (cases r)
+  case (fields prems concl)
+  have fin_prems: "finite (\<Union> (var_set_form ` set prems))"
+  proof (induction prems)
+    case Nil
+    then show ?case by simp
+  next
+    case (Cons p ps)
+    have fin_p: "finite (var_set_form p)"
+      by (induction p) auto
+    then show ?case
+      using Cons by auto
+  qed
+  have fin_concl: "finite (var_set_form concl)"
+    by (induction concl) auto
+  show ?thesis
+    using fields fin_prems fin_concl by simp
+qed
+
+(* -- End of general proofs -- *)
+
+locale de_morgan_frege =
+  fixes F :: dfrege
+  assumes conns_def: "conns (alphabet F) = {Top, Bot, Not, Or, And}"
+  and arity_def: "arity (alphabet F) = (\<lambda>c. case c of Top \<Rightarrow> 0 | Bot \<Rightarrow> 0 | Not \<Rightarrow> 1 | Or \<Rightarrow> 2 | And \<Rightarrow> 2)"
+  and conn_evals_def: "conn_evals (alphabet F) = (\<lambda> c. case c of
+    Top \<Rightarrow> (\<lambda>_. True)                \<comment> \<open>nullary: ignores input list\<close>
+  | Bot \<Rightarrow> (\<lambda>_. False)               \<comment> \<open>nullary\<close>
+  | Not \<Rightarrow> (\<lambda>args. case args of [x] \<Rightarrow> \<not> x | _ \<Rightarrow> undefined)
+  | Or  \<Rightarrow> (\<lambda>args. case args of [x, y] \<Rightarrow> x \<or> y | _ \<Rightarrow> undefined)
+  | And \<Rightarrow> (\<lambda>args. case args of [x, y] \<Rightarrow> x \<and> y | _ \<Rightarrow> undefined))"
+  and "frege_system F"
+begin
+abbreviation a where "a \<equiv> alphabet F"
 
 lemma len_sub_bound_by_proof:
   assumes "r \<in> rules F"
@@ -354,611 +231,108 @@ proof -
   thus ?thesis using len_proof_positive assms(4)
     by (metis assms(5) le_add2 less_one linorder_not_le max_absorb2 mult_is_0)
 qed
-
 end
-  
-locale de_morgan_sim =
+
+locale de_morgan_sim = 
   fixes F :: dfrege and F' :: dfrege
   assumes dm1: "de_morgan_frege F" and dm2: "de_morgan_frege F'"
-  and "modus_ponens \<in> rules F"
-  and "rule \<in> rules F \<longrightarrow> rule = modus_ponens \<or> prems rule = []"
 begin
 
-definition proof_of :: "dfrege \<Rightarrow> dproof \<Rightarrow> dformula \<Rightarrow> bool" where
-  "proof_of frege pr f \<longleftrightarrow> valid_proof frege pr \<and> assumptions pr = {} \<and> thesis pr = f"
-
-lemma rule_exists_proof:
-  assumes "r \<in> rules F'" and "f_rule = rule_to_taut r"
-shows "\<exists> pr. valid_proof F pr \<and>  assumptions pr = {} \<and> thesis pr = f_rule"
+lemma proof_exists_for_rule:
+  assumes "rule \<in> rules F"
+    shows "\<exists> pr. valid_proof F' pr \<and> assumptions pr = set (prems rule) \<and> thesis pr = concl rule"
 proof -
-  have "alphabet F = alphabet F'" 
-    using de_morgan_frege_def dm1 dm2 by force
-  hence all_val: "\<forall> val. eval (alphabet F) val f_rule"
-    using de_morgan_frege.sound_rule_gives_tautology[of F' r] assms dm2 by simp
-  have impl0:
-    "(\<forall> val. (\<forall>f\<in>{}. eval (alphabet F) val f) \<longrightarrow> eval (alphabet F) val f_rule)
-      \<longrightarrow> (\<exists>pr. valid_proof F pr \<and> assumptions pr = {} \<and> thesis pr = f_rule)"
-    using dm1 de_morgan_frege_def frege_system_def by blast
-  with impl0 all_val show ?thesis by simp
+  have "alphabet F = alphabet F'"
+    using dm1 dm2 de_morgan_frege_def by fastforce
+  hence val_sat: "\<forall> val. (\<forall> f \<in> set (prems rule). eval (alphabet F') val f) 
+                \<longrightarrow> eval (alphabet F') val (concl rule)"
+    using dm1 assms frege_system.sound sound_rule_def
+    by (metis de_morgan_frege_def)
+  have "(\<forall> val. (\<forall> f \<in> set (prems rule). eval (alphabet F') val f) \<longrightarrow> 
+                 eval (alphabet F') val (concl rule)) 
+                          \<longrightarrow> (\<exists> pr. valid_proof F' pr
+                                   \<and> assumptions pr = set (prems rule) 
+                                   \<and> thesis pr = concl rule)"
+    using dm2 frege_system_def de_morgan_frege_def by auto 
+  thus ?thesis using val_sat
+    by force
 qed
 
-lemma rule_proof_fun_F'_exists: "\<exists> f :: drule \<Rightarrow> dproof. \<forall> rule \<in> rules F'.
-          proof_of F (f rule) (rule_to_taut rule)"
+lemma rule_proof_fun_exists: "\<exists> f :: drule \<Rightarrow> dproof. \<forall> rule \<in> rules F.
+          valid_proof F' (f rule) \<and> 
+          assumptions (f rule) = set (prems rule) \<and> 
+          thesis (f rule) = concl rule"
+  by (meson proof_exists_for_rule)
+
+definition rule_proof_fun where
+  "rule_proof_fun = (SOME f. \<forall> rule \<in> rules F.
+          valid_proof F' (f rule) \<and> 
+          assumptions (f rule) = set (prems rule) \<and> 
+          thesis (f rule) = concl rule)"
+
+fun step_proof :: "drule \<Rightarrow> (string \<Rightarrow> dformula) \<Rightarrow> dproof" where
+  "step_proof rule sub = sub_proof sub (rule_proof_fun rule)"
+
+lemma step_proof_proves:
+  assumes "r \<in> rules F"
+  shows "valid_proof F' (step_proof r s) \<and>
+         assumptions (step_proof r s) = set (prems (sub_rule s r)) \<and>
+         thesis (step_proof r s) = concl (sub_rule s r)"
 proof -
-  have "\<forall> rule \<in> rules F'. \<exists> pr. proof_of F pr (rule_to_taut rule)"
-    using rule_exists_proof proof_of_def by simp
-  thus "\<exists> f. \<forall> rule \<in> rules F'. proof_of F (f rule) (rule_to_taut rule)" by meson
-qed
-
-definition rule_proof_fun_F' where
-  "rule_proof_fun_F' = (SOME f. \<forall> rule \<in> rules F'.
-          proof_of F (f rule) (rule_to_taut rule))"
-
-fun first_step :: "drule \<Rightarrow> (string \<Rightarrow> dformula) \<Rightarrow> dproof" where
-  "first_step rule sub = sub_proof sub (rule_proof_fun_F' rule)"
-
-lemma first_step_proves:
-  assumes "r \<in> rules F'"
-  shows "proof_of F (first_step r s) (rule_to_taut (sub_rule s r))"
-proof -
-  have sub_rule_to_taut:
-    "sub_formula sub (rule_to_taut rule) = rule_to_taut (sub_rule sub rule)"
-    for sub rule
-  proof (induction rule rule: rule_to_taut.induct)
-    case (1 c)
-    then show ?case by simp
-  next
-    case (2 f fs c)
-    then show ?case by simp
-  qed
-
   have ex_fun:
-    "\<exists>f :: drule \<Rightarrow> dproof. \<forall>rule \<in> rules F'. proof_of F (f rule) (rule_to_taut rule)"
-    using rule_proof_fun_F'_exists .
+    "\<exists>f :: drule \<Rightarrow> dproof. \<forall>rule \<in> rules F.
+      valid_proof F' (f rule) \<and> assumptions (f rule) = set (prems rule) \<and> thesis (f rule) = concl rule"
+    using rule_proof_fun_exists .
   have fun_prop:
-    "\<forall>rule \<in> rules F'. proof_of F (rule_proof_fun_F' rule) (rule_to_taut rule)"
-    unfolding rule_proof_fun_F'_def
-    by (rule someI_ex[OF ex_fun])
-
-  have base_proof: "proof_of F (rule_proof_fun_F' r) (rule_to_taut r)"
-    using fun_prop assms by blast
-  then have base_valid: "valid_proof F (rule_proof_fun_F' r)"
-    and base_assm: "assumptions (rule_proof_fun_F' r) = {}"
-    and base_th: "thesis (rule_proof_fun_F' r) = rule_to_taut r"
-    unfolding proof_of_def by auto
-
-  have sub_valid: "valid_proof F (sub_proof s (rule_proof_fun_F' r))"
-    using frege_system.proof_substitution dm1 base_valid de_morgan_frege_def by auto
-  have sub_assm: "assumptions (sub_proof s (rule_proof_fun_F' r)) = {}"
+    "\<forall>rule \<in> rules F.
+      valid_proof F' (rule_proof_fun rule) \<and>
+      assumptions (rule_proof_fun rule) = set (prems rule) \<and>
+      thesis (rule_proof_fun rule) = concl rule"
+    unfolding rule_proof_fun_def by (rule someI_ex[OF ex_fun])
+  then have base:
+    "valid_proof F' (rule_proof_fun r) \<and>
+     assumptions (rule_proof_fun r) = set (prems r) \<and>
+     thesis (rule_proof_fun r) = concl r"
+    using assms by blast
+  then have base_valid: "valid_proof F' (rule_proof_fun r)"
+    and base_assm: "assumptions (rule_proof_fun r) = set (prems r)"
+    and base_th: "thesis (rule_proof_fun r) = concl r"
+    by auto
+  have fsys: "frege_system F'"
+    using dm2 unfolding de_morgan_frege_def by simp
+  interpret fs: frege_system F'
+    by (rule fsys)
+  have sub_valid: "valid_proof F' (step_proof r s)"
+    unfolding step_proof.simps using fs.proof_substitution[OF base_valid] .
+  have sub_assm: "assumptions (step_proof r s) = set (prems (sub_rule s r))"
     using base_assm by simp
-  have sub_th: "thesis (sub_proof s (rule_proof_fun_F' r)) = rule_to_taut (sub_rule s r)"
-    using base_th sub_rule_to_taut[of s r] by simp
-
+  have sub_th: "thesis (step_proof r s) = concl (sub_rule s r)"
+    using base_th by simp
   show ?thesis
-    unfolding first_step.simps proof_of_def
-    using sub_valid sub_assm sub_th by blast
-qed
-
-lemma var_set_rule_finite:
-  shows "finite (var_set_rule r)"
-proof (cases r)
-  case (fields prems concl)
-  have fin_prems: "finite (\<Union> (var_set_form ` set prems))"
-  proof (induction prems)
-    case Nil
-    then show ?case by simp
-  next
-    case (Cons p ps)
-    have fin_p: "finite (var_set_form p)"
-      by (induction p) auto
-    then show ?case
-      using Cons by auto
-  qed
-  have fin_concl: "finite (var_set_form concl)"
-    by (induction concl) auto
-  show ?thesis
-    using fields fin_prems fin_concl by simp
-qed
-
-lemma first_step_is_bound: 
-  shows "\<exists> g :: (drule \<Rightarrow> nat poly). \<forall> rule \<in> rules F'. \<forall>  sub. 
-            rule_restricted_sub rule sub \<longrightarrow> 
-            len_proof (first_step rule sub) \<le> poly (g rule) (len_sub (var_set_rule rule) sub)"
-proof -
-  let ?g = "\<lambda>rule. [:0, len_proof (rule_proof_fun_F' rule):]"
-
-  have bound_per_rule:
-    "\<forall>rule \<in> rules F'. \<forall>sub.
-      rule_restricted_sub rule sub \<longrightarrow>
-      len_proof (first_step rule sub) \<le> poly (?g rule) (len_sub (var_set_rule rule) sub)"
-  proof (intro ballI allI impI)
-    fix rule sub
-    assume "rule \<in> rules F'"
-    assume rsub: "rule_restricted_sub rule sub"
-    have restricted_sub: "\<forall>v. v \<notin> var_set_rule rule \<longrightarrow> sub v = Atom v"
-      using rsub unfolding rule_restricted_sub_def by simp
-
-    have bound:
-      "len_proof (first_step rule sub)
-       \<le> len_proof (rule_proof_fun_F' rule) * len_sub (var_set_rule rule) sub"
-      unfolding first_step.simps
-      using sub_proof_bound[of "var_set_rule rule" sub "rule_proof_fun_F' rule"]
-      using var_set_rule_finite[of rule] restricted_sub by simp
-
-    have poly_eval:
-      "poly (?g rule) (len_sub (var_set_rule rule) sub) =
-       len_proof (rule_proof_fun_F' rule) * len_sub (var_set_rule rule) sub"
-      by simp
-
-    show "len_proof (first_step rule sub) \<le> poly (?g rule) (len_sub (var_set_rule rule) sub)"
-      using bound poly_eval by (simp add: algebra_simps)
-  qed
-
-  show ?thesis using bound_per_rule by meson
-qed
-
-(* peel only returns Some if the input formula is equal to the expected end, or we can peel off
-with modus ponens and arrive at the expected formula. *)
-fun peel :: "dformula \<Rightarrow> dformula \<Rightarrow> dproof option" where
-  "peel x y =
-   (if x = y then Some \<lparr>assumptions = {x}, thesis = x, steps = [x]\<rparr>
-    else case x of
-      Atom _ \<Rightarrow> None
-    | Conn c fs \<Rightarrow>
-        (if c = Or then
-           (case fs of
-              [Conn d [a], b] \<Rightarrow>
-                (if d = Not then
-                   (case peel b y of
-                      Some p \<Rightarrow> Some (combine_proofs \<lparr>assumptions = {x, a}, thesis = b, steps = [x, a, b]\<rparr> p)
-                    | None \<Rightarrow> None)
-                 else None)
-            | _ \<Rightarrow> None)
-         else None))"
-
-(* We prove from the flattened rule the conclusion, peeling with modus ponens each implication.
-Note that we add each premise to assumptions and then include it as a step to immediately
-derive from it the peeled formula.*)
-fun second_step :: "drule \<Rightarrow> dproof" where
-  "second_step rule = (case peel (rule_to_taut rule) (concl rule) of
-                      Some p \<Rightarrow> p
-                    | None \<Rightarrow> undefined)"
-
-lemma peel_valid: "peel x y = Some p \<longrightarrow> valid_proof F p"
-proof (induction x arbitrary: y p)
-  case (Atom a)
-  show ?case
-    by (auto simp: valid_proof_def split: if_splits)
-next
-  case (Conn c fs)
-  show ?case
-  proof
-    assume peel_some: "peel (Conn c fs) y = Some p"
-    show "valid_proof F p"
-    proof (cases "Conn c fs = y")
-      case True
-      with peel_some show ?thesis
-        by (auto simp: valid_proof_def)
-    next
-      case False
-      obtain a v q where
-        c_def: "c = Or"
-        and fs_def: "fs = [Conn Not [a], v]"
-        and rec_v: "peel v y = Some q"
-        using peel_some False
-        by (cases fs) (auto split: option.splits if_splits formula.splits list.splits)
-      have p_def: "p = combine_proofs \<lparr>assumptions = {Conn c fs, a}, thesis = v, steps = [Conn c fs, a, v]\<rparr> q"
-        using peel_some False c_def fs_def rec_v
-        by simp
-     
-
-      let ?sub = "\<lambda>s. if s = ''P'' then a else if s = ''Q'' then v else Atom s"
-
-      (* \<not>a \<or> v, a \<longrightarrow> v *)
-      have der_v: "derived (rules F) [Conn c fs, a] v"
-      proof -
-        have "modus_ponens \<in> rules F"
-          using de_morgan_sim_axioms unfolding de_morgan_sim_def by auto
-        moreover have
-          "let sub_r = sub_rule ?sub modus_ponens in
-             concl sub_r = v \<and>
-             (\<forall>f1\<in>set (prems sub_r). \<exists>f2\<in>set [Conn c fs, a]. f1 = f2)"
-          unfolding modus_ponens_def
-          using c_def fs_def
-          by simp
-        ultimately show ?thesis
-          unfolding derived_def
-          by (intro bexI[of _ modus_ponens] exI[of _ ?sub]) simp
-      qed
-
-      have seed_valid:
-        "valid_proof F \<lparr>assumptions = {Conn c fs, a}, thesis = v, steps = [Conn c fs, a, v]\<rparr>"
-      proof -
-        have steps_ok:
-          "\<forall>i<length [Conn c fs, a, v].
-             [Conn c fs, a, v] ! i \<in> {Conn c fs, a} \<or>
-             derived (rules F) (take i [Conn c fs, a, v]) ([Conn c fs, a, v] ! i)"
-        proof (intro allI impI)
-          fix i
-          assume i_lt: "i < length [Conn c fs, a, v]"
-          show "[Conn c fs, a, v] ! i \<in> {Conn c fs, a} \<or>
-                derived (rules F) (take i [Conn c fs, a, v]) ([Conn c fs, a, v] ! i)"
-          proof (cases i)
-            case 0
-            then show ?thesis by simp
-          next
-            case (Suc j)
-            have i_suc: "i = Suc j"
-              using Suc by simp
-            then show ?thesis
-            proof (cases j)
-              case 0
-              then show ?thesis using Suc by simp
-            next
-              case (Suc k)
-              have i_eq: "i = Suc (Suc k)"
-                using i_suc Suc by simp
-              have "k < 1"
-                using i_lt i_eq by simp
-              then have "k = 0"
-                by simp
-              have i_two: "i = 2"
-                using i_suc Suc \<open>k = 0\<close> by simp
-              show ?thesis
-                using der_v i_two by simp
-            qed
-          qed
-        qed
-        show ?thesis
-          unfolding valid_proof_def
-          using steps_ok by simp
-      qed
-
-      have v_in_fs: "v \<in> set fs"
-        using fs_def by simp
-      have q_valid: "valid_proof F q"
-        using Conn.IH[OF v_in_fs, of y q] rec_v by simp
-
-      have fsys: "frege_system F"
-        using dm1 unfolding de_morgan_frege_def by simp
-      have comb_valid:
-        "valid_proof F (combine_proofs \<lparr>assumptions = {Conn c fs, a}, thesis = v, steps = [Conn c fs, a, v]\<rparr> q)"
-        using fsys seed_valid q_valid frege_system.combining_valid_proofs by blast
-
-      show ?thesis
-        using p_def comb_valid by simp
-    qed
-  qed
-qed
-
-lemma r_t_t_peelable: "\<exists> p. peel (rule_to_taut rule) (concl rule) = Some p"
-proof (induction "prems rule" arbitrary: rule)
-  case Nil
-  hence "rule = \<lparr>prems = [], concl = concl rule\<rparr>" by simp
-  hence "rule_to_taut rule = rule_to_taut \<lparr>prems = [], concl = concl rule\<rparr>" by simp
-  hence "rule_to_taut rule = concl rule" by simp
-  hence "\<exists> p. peel (rule_to_taut rule) (concl rule) = Some p" by auto
-  thus ?case by simp
-next
-  case (Cons f fs)
-  have rule_eq: "rule = \<lparr>prems = f # fs, concl = concl rule\<rparr>"
-    using Cons by simp
-  let ?tail = "rule_to_taut \<lparr>prems = fs, concl = concl rule\<rparr>"
-  have "rule_to_taut rule = rule_to_taut \<lparr>prems = f # fs, concl = concl rule\<rparr>" 
-    using rule_eq by simp
-  hence rt_def: "rule_to_taut rule = Conn Or [Conn Not [f], ?tail]"
-    using rule_to_taut.simps by simp
-  have tail_peelable: "\<exists>q. peel ?tail (concl rule) = Some q"
-    using Cons by (metis rule.select_convs(1,2))
-  then obtain q where q_def: "peel ?tail (concl rule) = Some q"
-    by blast
-
-  show ?case
-  proof (cases "rule_to_taut rule = concl rule")
-    case True
-    then show ?thesis by auto
-  next
-    case False
-    have "peel (rule_to_taut rule) (concl rule) =
-          Some (combine_proofs
-                  \<lparr>assumptions = {rule_to_taut rule, f},
-                   thesis = ?tail,
-                   steps = [rule_to_taut rule, f, ?tail]\<rparr> q)"
-      using rt_def False q_def by simp
-    then show ?thesis by blast
-  qed
-qed
-
-lemma premise_shorter_than_rule_to_taut_aux:
-  assumes "x \<in> set ps"
-  shows "len_formula x < len_formula (rule_to_taut \<lparr>prems = ps, concl = c\<rparr>)"
-  using assms
-proof (induction ps)
-  case Nil
-  then show ?case by simp
-next
-  case (Cons f fs)
-  show ?case
-  proof (cases "x = f")
-    case True
-    then show ?thesis by simp
-  next
-    case False
-    then have x_in_fs: "x \<in> set fs"
-      using Cons.prems by simp
-    have ih: "len_formula x < len_formula (rule_to_taut \<lparr>prems = fs, concl = c\<rparr>)"
-      using Cons.IH[OF x_in_fs] .
-    have tail_lt:
-      "len_formula (rule_to_taut \<lparr>prems = fs, concl = c\<rparr>) <
-       len_formula (rule_to_taut \<lparr>prems = f # fs, concl = c\<rparr>)"
-      by simp
-    from ih tail_lt show ?thesis by arith
-  qed
-qed
-
-lemma premise_shorter_than_rule_to_taut:
-  assumes "x \<in> set (prems r)"
-  shows "len_formula x < len_formula (rule_to_taut r)"
-proof (cases r)
-  case (fields prems concl)
-  then show ?thesis
-    using premise_shorter_than_rule_to_taut_aux[of x prems concl] assms by simp
-qed
-
-lemma peel_thesis:
-  assumes "peel x y = Some p"
-  shows "thesis p = y"
-  using assms
-proof (induction x arbitrary: y p)
-  case (Atom a)
-  then show ?case
-    by (auto split: if_splits)
-next
-  case (Conn c fs)
-  show ?case
-  proof (cases "Conn c fs = y")
-    case True
-    have "p = \<lparr>assumptions = {y}, thesis = y, steps = [y]\<rparr>"
-      using Conn.prems True by simp
-    then show ?thesis
-      by simp
-  next
-    case False
-    obtain d a b q where
-      c_def: "c = Or"
-      and fs_def: "fs = [Conn d [a], b]"
-      and d_def: "d = Not"
-      and rec: "peel b y = Some q"
-      and p_def: "p = combine_proofs \<lparr>assumptions = {Conn c fs, a}, thesis = b, steps = [Conn c fs, a, b]\<rparr> q"
-      using Conn.prems False
-      by (cases fs) (auto split: option.splits if_splits formula.splits list.splits)
-
-    show ?thesis
-      using p_def Conn.IH[OF _ rec] fs_def by simp
-  qed
-qed
-
-lemma rule_to_taut_notin_prems:
-  shows "rule_to_taut r \<notin> set (prems r)"
-proof
-  assume "rule_to_taut r \<in> set (prems r)"
-  then have "len_formula (rule_to_taut r) < len_formula (rule_to_taut r)"
-    using premise_shorter_than_rule_to_taut[of "rule_to_taut r" r] by simp
-  then show False by simp
-qed
-
-lemma peel_rule_to_taut_assumptions:
-  assumes "peel (rule_to_taut rule) (concl rule) = Some p"
-  shows "assumptions p = {rule_to_taut rule} \<union> set (prems rule)"
-proof -
-  obtain ps c where rule_def: "rule = \<lparr>prems = ps, concl = c\<rparr>"
-    by (cases rule) auto
-  have assm0: "peel (rule_to_taut \<lparr>prems = ps, concl = c\<rparr>) c = Some p"
-    using assms rule_def by simp
-  have "assumptions p = {rule_to_taut \<lparr>prems = ps, concl = c\<rparr>} \<union> set ps"
-    using assm0
-  proof (induction ps arbitrary: p)
-    case Nil
-    then have p_def: "p = \<lparr>assumptions = {c}, thesis = c, steps = [c]\<rparr>"
-      by simp
-    then show ?case by simp
-  next
-    case (Cons f fs)
-    let ?tail = "\<lparr>prems = fs, concl = c\<rparr>"
-    have rt_def: "rule_to_taut \<lparr>prems = f # fs, concl = c\<rparr> = Conn Or [Conn Not [f], rule_to_taut ?tail]"
-      by simp
-    have tail_ge: "len_formula (rule_to_taut ?tail) \<ge> len_formula c"
-    proof (induction fs)
-      case Nil
-      then show ?case by simp
-    next
-      case (Cons g gs)
-      then show ?case by simp
-    qed
-    have rt_ne_c: "rule_to_taut \<lparr>prems = f # fs, concl = c\<rparr> \<noteq> c"
-    proof
-      assume eq: "rule_to_taut \<lparr>prems = f # fs, concl = c\<rparr> = c"
-      have "len_formula (rule_to_taut \<lparr>prems = f # fs, concl = c\<rparr>) > len_formula c"
-        using tail_ge by simp
-      moreover have "len_formula (rule_to_taut \<lparr>prems = f # fs, concl = c\<rparr>) = len_formula c"
-        using eq by simp
-      ultimately show False by simp
-    qed
-    from Cons.prems obtain q where
-      q_def: "peel (rule_to_taut ?tail) c = Some q"
-      and p_def: "p = combine_proofs \<lparr>assumptions = {rule_to_taut \<lparr>prems = f # fs, concl = c\<rparr>, f},
-                                      thesis = rule_to_taut ?tail,
-                                      steps = [rule_to_taut \<lparr>prems = f # fs, concl = c\<rparr>, f, rule_to_taut ?tail]\<rparr> q"
-      using rt_def rt_ne_c by (auto split: option.splits if_splits)
-    have q_assm: "assumptions q = {rule_to_taut ?tail} \<union> set fs"
-      using Cons.IH[OF q_def] by simp
-    have tail_notin_fs: "rule_to_taut ?tail \<notin> set fs"
-      using rule_to_taut_notin_prems[of ?tail] by simp
-    show ?case
-      using p_def q_assm tail_notin_fs by auto
-  qed
-  then show ?thesis
-    using rule_def by simp
-qed
-
-lemma second_step_proves:
-  fixes rule :: drule
-  assumes "pr = second_step rule"
-  shows "valid_proof F pr \<and> 
-         assumptions pr = {rule_to_taut rule} \<union> set (prems rule) \<and> 
-         thesis pr = concl rule"
-proof -
-  obtain p where peel_res: "peel (rule_to_taut rule) (concl rule) = Some p"
-    using r_t_t_peelable by blast
-  have pr_eq: "pr = p"
-    using assms peel_res by simp
-  show ?thesis
-    using pr_eq peel_res peel_valid peel_rule_to_taut_assumptions peel_thesis by auto
-qed
-
-lemma peel_bound:
-  assumes "peel x y = Some p"
-  shows "len_proof p \<le> (len_formula x)^2"
-  using assms
-proof (induction x arbitrary: y p)
-  case (Atom x)
-  assume "peel (Atom x) y = Some p"
-  hence "y = Atom x" using peel.elims by fastforce
-  hence "peel (Atom x) y = Some \<lparr>assumptions = {Atom x}, thesis = Atom x, steps = [Atom x]\<rparr>" by simp
-  hence "len_proof p = sum_list (map len_formula [Atom x])" using Atom by auto
-  thus ?case by simp
-next
-  case (Conn c fs)
-  show ?case
-  proof (cases "Conn c fs = y")
-    case True
-    hence "peel (Conn c fs) y = Some \<lparr>assumptions = {Conn c fs}, thesis = Conn c fs, steps = [Conn c fs]\<rparr>" 
-      by simp
-    hence "len_proof p = sum_list (map len_formula [Conn c fs])" using Conn.prems by auto
-    hence "len_proof p = len_formula (Conn c fs)" by simp
-    thus ?thesis
-      by (simp add: power2_nat_le_imp_le) 
-  next
-    case False
-    hence "\<exists> a b. Conn c fs = Conn Or [Conn Not [a], b]"
-      using Conn.prems
-      by (cases fs) (auto split: option.splits if_splits formula.splits list.splits)
-    obtain a b q where
-      c_def: "c = Or"
-      and fs_def: "fs = [Conn Not [a], b]"
-      and rec: "peel b y = Some q"
-      and p_def: "p = combine_proofs \<lparr>assumptions = {Conn c fs, a}, thesis = b, steps = [Conn c fs, a, b]\<rparr> q"
-      using Conn.prems False
-      by (cases fs) (auto split: option.splits if_splits formula.splits list.splits)
-    have b_in: "b \<in> set fs"
-      using fs_def by simp
-    have IHb: "len_proof q \<le> (len_formula b)^2"
-      using Conn.IH[OF b_in rec] by simp
-    have p_len: "len_proof p = len_formula (Conn c fs) + len_formula a + len_formula b + len_proof q"
-      using p_def by simp
-    have len_x: "len_formula (Conn c fs) = len_formula a + len_formula b + 2"
-      using c_def fs_def by simp
-    have bound1: "len_proof p \<le> len_formula (Conn c fs) + len_formula a + len_formula b + (len_formula b)^2"
-      using p_len IHb by simp
-    have bound2:
-      "len_formula (Conn c fs) + len_formula a + len_formula b + (len_formula b)^2
-       \<le> (len_formula b)^2 + 4 * len_formula a + 4 * len_formula b + 4"
-      using len_x by linarith
-    have bound3:
-      "(len_formula b)^2 + 4 * len_formula a + 4 * len_formula b + 4
-       \<le> (len_formula (Conn c fs))^2"
-      using len_x by (simp add: power2_eq_square algebra_simps)
-    have "len_proof p \<le> (len_formula (Conn c fs))^2"
-      using bound1 bound2 bound3 by (meson order_trans)
-    thus ?thesis by simp
-  qed
+    using sub_valid sub_assm sub_th by simp
 qed
 
 definition choose_rule_sub where
   "choose_rule_sub frege i pr =
      (SOME (r,s). r \<in> rules frege \<and> derived_with i pr r s \<and> rule_restricted_sub r s)"
 
-definition sim_right_step :: "dproof \<Rightarrow> nat \<Rightarrow> dproof \<Rightarrow> dproof" where
-  "sim_right_step pr i acc =
+definition sim_step :: "dproof \<Rightarrow> nat \<Rightarrow> dproof \<Rightarrow> dproof" where
+  "sim_step pr i acc =
     (let step = (steps pr) ! i in
       if step \<in> assumptions pr then 
         combine_proofs acc \<lparr>assumptions = {}, thesis = step, steps = [step]\<rparr>
       else
-        let (r, s) = choose_rule_sub F' i pr in
-        let pr1 = first_step r s;
-            pr2 = second_step (sub_rule s r)
-        in combine_proofs acc (combine_proofs pr1 pr2))"
+        let (r, s) = choose_rule_sub F i pr in
+        let pr = step_proof r s
+        in combine_proofs acc pr)"
 
-definition sim_right :: "dproof \<Rightarrow> dformula \<Rightarrow> dproof" where
-  "sim_right pr th =
-     fold (sim_right_step pr)
+definition sim :: "dproof \<Rightarrow> dformula \<Rightarrow> dproof" where
+  "sim pr th =
+     fold (sim_step pr)
        [0..<length (steps pr)]
        \<lparr>assumptions = assumptions pr,
         thesis = th,
         steps = []\<rparr>"
-
-lemma sim_right_single_der:
-  fixes r :: drule
-  and s :: "string \<Rightarrow> dformula"
-  assumes r_in: "r \<in> rules F'"
-  assumes "pr = combine_proofs (first_step r s) (second_step (sub_rule s r))"
-  shows "valid_proof F pr \<and> 
-         thesis pr = concl (sub_rule s r) \<and> 
-         assumptions pr = set (prems (sub_rule s r)) - set (steps (first_step r s))"
-proof -
-  let ?rsub = "sub_rule s r"
-  let ?pr1 = "first_step r s"
-  let ?pr2 = "second_step ?rsub"
-
-  have pr1_proof: "proof_of F ?pr1 (rule_to_taut ?rsub)"
-    using first_step_proves[OF r_in] .
-  then have pr1_valid: "valid_proof F ?pr1"
-    and pr1_assm: "assumptions ?pr1 = {}"
-    and pr1_th: "thesis ?pr1 = rule_to_taut ?rsub"
-    unfolding proof_of_def by auto
-
-  have pr2_props:
-    "valid_proof F ?pr2 \<and>
-     assumptions ?pr2 = {rule_to_taut ?rsub} \<union> set (prems ?rsub) \<and>
-     thesis ?pr2 = concl ?rsub"
-    using second_step_proves[of ?pr2 ?rsub] by simp
-  then have pr2_valid: "valid_proof F ?pr2"
-    and pr2_assm: "assumptions ?pr2 = {rule_to_taut ?rsub} \<union> set (prems ?rsub)"
-    and pr2_th: "thesis ?pr2 = concl ?rsub"
-    by auto
-
-  have fsys: "frege_system F"
-    using dm1 unfolding de_morgan_frege_def by simp
-  have pr_valid: "valid_proof F pr"
-    using assms(2) pr1_valid pr2_valid fsys frege_system.combining_valid_proofs by blast
-  have pr_thesis: "thesis pr = concl ?rsub"
-    using assms(2) pr2_th by simp
-
-  have pr1_nonempty: "steps ?pr1 \<noteq> []"
-    using pr1_valid unfolding valid_proof_def by simp
-  have taut_in_steps: "rule_to_taut ?rsub \<in> set (steps ?pr1)"
-  proof -
-    have "thesis ?pr1 = last (steps ?pr1)"
-      using pr1_valid unfolding valid_proof_def by simp
-    then have eq_last: "rule_to_taut ?rsub = last (steps ?pr1)"
-      using pr1_th by simp
-    have "last (steps ?pr1) \<in> set (steps ?pr1)"
-      using pr1_nonempty by (rule last_in_set)
-    then show ?thesis
-      by (simp only: eq_last)
-  qed
-
-  have taut_notin_prems: "rule_to_taut ?rsub \<notin> set (prems ?rsub)"
-    using rule_to_taut_notin_prems[of ?rsub] .
-  have pr_assms0:
-    "assumptions pr = ({rule_to_taut ?rsub} \<union> set (prems ?rsub)) - set (steps ?pr1)"
-    using assms(2) pr1_assm pr2_assm by simp
-  have pr_assms: "assumptions pr = set (prems ?rsub) - set (steps ?pr1)"
-    using pr_assms0 taut_in_steps taut_notin_prems by auto
-
-  show ?thesis
-    using pr_valid pr_thesis pr_assms by simp
-qed
 
 lemma sub_formula_agree:
   "sub_formula s1 f = sub_formula s2 f"
@@ -973,12 +347,14 @@ next
   then show ?case by simp
 qed
 
+
 lemma sub_rule_agree:
   "sub_rule s1 r = sub_rule s2 r"
   if "\<forall>v \<in> var_set_rule r. s1 v = s2 v"
   for s1 s2 :: "string \<Rightarrow> dformula" and r
 using that
 by (cases r) (auto intro: sub_formula_agree)
+
 
 lemma choose_rule_sub_props:
   assumes "\<exists>r s. r \<in> rules G \<and> derived_with i p r s"
@@ -1005,1016 +381,8 @@ proof -
     unfolding choose_rule_sub_def by (cases "SOME rs. ?P rs") auto
 qed
 
-lemma sim_right_proves:
-  fixes pr :: dproof
-  assumes "valid_proof F' pr'"
-  and "assumptions pr' = {}"
-  and "pr = sim_right pr' (thesis pr')"
-shows "valid_proof F pr \<and> thesis pr = thesis pr' \<and> assumptions pr = {}"
-proof -
-  let ?init = "\<lparr>assumptions = assumptions pr', thesis = thesis pr', steps = []\<rparr>"
-  let ?acc = "\<lambda>k. fold (sim_right_step pr') [0..<k] ?init"
-  let ?n = "length (steps pr')"
 
-  have choose_rule_sub_props:
-    "\<exists>r s. r \<in> rules F' \<and> derived_with i p r s
-     \<Longrightarrow> fst (choose_rule_sub F' i p) \<in> rules F' \<and>
-         derived_with i p (fst (choose_rule_sub F' i p)) (snd (choose_rule_sub F' i p)) \<and>
-         rule_restricted_sub (fst (choose_rule_sub F' i p)) (snd (choose_rule_sub F' i p))"
-    for i p
-  proof -
-    assume ex: "\<exists>r s. r \<in> rules F' \<and> derived_with i p r s"
-    then obtain r s where r_in: "r \<in> rules F'" and dwith: "derived_with i p r s"
-      by blast
-    define s' where "s' = (\<lambda>v. if v \<in> var_set_rule r then s v else Atom v)"
-    have rs_eq: "sub_rule s' r = sub_rule s r"
-      unfolding s'_def
-      by (rule sub_rule_agree) auto
-    have dwith': "derived_with i p r s'"
-      using dwith unfolding derived_with_def rs_eq by simp
-    have rsub': "rule_restricted_sub r s'"
-      unfolding rule_restricted_sub_def s'_def by simp
-    let ?P = "\<lambda>rs :: drule \<times> (string \<Rightarrow> dformula).
-      case rs of (r, s) \<Rightarrow> r \<in> rules F' \<and> derived_with i p r s \<and> rule_restricted_sub r s"
-    have ex_pair: "\<exists>rs. ?P rs"
-      using r_in dwith' rsub' by force
-    have "?P (SOME rs. ?P rs)"
-      by (rule someI_ex[OF ex_pair])
-    then show "fst (choose_rule_sub F' i p) \<in> rules F' \<and>
-               derived_with i p (fst (choose_rule_sub F' i p)) (snd (choose_rule_sub F' i p)) \<and>
-               rule_restricted_sub (fst (choose_rule_sub F' i p)) (snd (choose_rule_sub F' i p))"
-      unfolding choose_rule_sub_def
-      by (cases "SOME rs. ?P rs") auto
-  qed
-
-  have prefix_inv:
-    "\<forall>k\<le>?n.
-      assumptions (?acc k) = {} \<and>
-      set (take k (steps pr')) \<subseteq> set (steps (?acc k)) \<and>
-      (k = 0 \<or> (valid_proof F (?acc k) \<and> thesis (?acc k) = steps pr' ! (k - 1)))"
-  proof (intro allI impI)
-    fix k
-    assume k_le: "k \<le> ?n"
-    show "assumptions (?acc k) = {} \<and>
-          set (take k (steps pr')) \<subseteq> set (steps (?acc k)) \<and>
-          (k = 0 \<or> (valid_proof F (?acc k) \<and> thesis (?acc k) = steps pr' ! (k - 1)))"
-      using k_le
-    proof (induction k)
-      case 0
-      then show ?case
-        using assms(2) by simp
-    next
-      case (Suc k)
-      have k_le: "k \<le> ?n" using Suc.prems by simp
-      have k_lt: "k < ?n" using Suc.prems by simp
-      have ih:
-        "assumptions (?acc k) = {} \<and>
-         set (take k (steps pr')) \<subseteq> set (steps (?acc k)) \<and>
-         (k = 0 \<or> (valid_proof F (?acc k) \<and> thesis (?acc k) = steps pr' ! (k - 1)))"
-        using Suc.IH[OF k_le] .
-      then have acc_assm0: "assumptions (?acc k) = {}" by simp
-      from ih have take_k_in_steps: "set (take k (steps pr')) \<subseteq> set (steps (?acc k))"
-        by simp
-
-      have step_not_assm: "steps pr' ! k \<notin> assumptions pr'"
-        using assms(2) k_lt by simp
-      have der_k: "derived (rules F') (take k (steps pr')) (steps pr' ! k)"
-        using assms(1) k_lt step_not_assm
-        unfolding valid_proof_def by blast
-
-      have ex_rs: "\<exists>r s. r \<in> rules F' \<and> derived_with k pr' r s"
-        using der_k unfolding derived_def derived_with_def by (meson k_lt)
-      have choose_props:
-        "fst (choose_rule_sub F' k pr') \<in> rules F' \<and>
-         derived_with k pr' (fst (choose_rule_sub F' k pr')) (snd (choose_rule_sub F' k pr')) \<and>
-         rule_restricted_sub (fst (choose_rule_sub F' k pr')) (snd (choose_rule_sub F' k pr'))"
-        using choose_rule_sub_props[OF ex_rs] .
-      let ?r = "fst (choose_rule_sub F' k pr')"
-      let ?s = "snd (choose_rule_sub F' k pr')"
-      have r_in: "?r \<in> rules F'" using choose_props by simp
-      have dwith: "derived_with k pr' ?r ?s" using choose_props by simp
-      have concl_step: "concl (sub_rule ?s ?r) = steps pr' ! k"
-        using dwith unfolding derived_with_def by (simp add: Let_def)
-      have prems_in_takek:
-        "\<forall>f1 \<in> set (prems (sub_rule ?s ?r)). \<exists>f2 \<in> set (take k (steps pr')). f1 = f2"
-        using dwith unfolding derived_with_def by (simp add: Let_def)
-
-      let ?inner = "combine_proofs (first_step ?r ?s) (second_step (sub_rule ?s ?r))"
-      have inner_props:
-        "valid_proof F ?inner \<and>
-         thesis ?inner = concl (sub_rule ?s ?r) \<and>
-         assumptions ?inner = set (prems (sub_rule ?s ?r)) - set (steps (first_step ?r ?s))"
-      proof (rule sim_right_single_der[OF r_in])
-        show "?inner = combine_proofs (first_step ?r ?s) (second_step (sub_rule ?s ?r))"
-          by simp
-      qed
-      then have inner_valid: "valid_proof F ?inner"
-        and inner_th: "thesis ?inner = concl (sub_rule ?s ?r)"
-        and inner_assm:
-          "assumptions ?inner = set (prems (sub_rule ?s ?r)) - set (steps (first_step ?r ?s))"
-        by auto
-      have inner_assm_subset_takek: "assumptions ?inner \<subseteq> set (take k (steps pr'))"
-        using inner_assm prems_in_takek by auto
-
-      have acc_suc:
-        "?acc (Suc k) = sim_right_step pr' k (?acc k)"
-        by (simp add: atLeastLessThanSuc)
-      have step_eq:
-        "sim_right_step pr' k (?acc k) = combine_proofs (?acc k) ?inner"
-      proof -
-        have "sim_right_step pr' k (?acc k) =
-              (let (r, s) = choose_rule_sub F' k pr' in
-               let pr1 = first_step r s;
-                   pr2 = second_step (sub_rule s r)
-               in combine_proofs (?acc k) (combine_proofs pr1 pr2))"
-          unfolding sim_right_step_def
-          using step_not_assm
-          by (simp add: Let_def)
-        then have eq1:
-          "sim_right_step pr' k (?acc k) =
-           (let (r, s) = choose_rule_sub F' k pr' in
-            let pr1 = first_step r s;
-                pr2 = second_step (sub_rule s r)
-            in combine_proofs (?acc k) (combine_proofs pr1 pr2))"
-          .
-        obtain a b where ch: "choose_rule_sub F' k pr' = (a, b)"
-          by (cases "choose_rule_sub F' k pr'") auto
-        have "sim_right_step pr' k (?acc k) =
-              (let (r, s) = (a, b) in
-               let pr1 = first_step r s;
-                   pr2 = second_step (sub_rule s r)
-               in combine_proofs (?acc k) (combine_proofs pr1 pr2))"
-          using eq1 ch by simp
-        then have "sim_right_step pr' k (?acc k) =
-              combine_proofs (?acc k) (combine_proofs (first_step a b) (second_step (sub_rule b a)))"
-          by (simp add: Let_def)
-        also have "... = combine_proofs (?acc k) ?inner"
-          using ch by (simp del: second_step.simps peel.simps)
-        finally show ?thesis .
-      qed
-      have new_eq:
-        "?acc (Suc k) = combine_proofs (?acc k) ?inner"
-        using acc_suc step_eq by simp
-
-      have assm_suc: "assumptions (?acc (Suc k)) = {}"
-      proof -
-        have "assumptions (?acc (Suc k)) =
-              assumptions (?acc k) \<union> (assumptions ?inner - set (steps (?acc k)))"
-          using new_eq by simp
-        also have "... = {} \<union> (assumptions ?inner - set (steps (?acc k)))"
-          using acc_assm0 by simp
-        also have "... = {}"
-        proof -
-          have "assumptions ?inner \<subseteq> set (steps (?acc k))"
-            using inner_assm_subset_takek take_k_in_steps by blast
-          then show ?thesis by auto
-        qed
-        finally show ?thesis by simp
-      qed
-
-      have step_in_inner_steps: "steps pr' ! k \<in> set (steps ?inner)"
-      proof -
-        have inner_nz: "steps ?inner \<noteq> []"
-          using inner_valid unfolding valid_proof_def by simp
-        have th_last: "thesis ?inner = last (steps ?inner)"
-          using inner_valid unfolding valid_proof_def by simp
-        have "last (steps ?inner) = thesis ?inner"
-          using th_last by simp
-        also have "... = concl (sub_rule ?s ?r)"
-          using inner_th by simp
-        also have "... = steps pr' ! k"
-          using concl_step by simp
-        finally have "steps pr' ! k = last (steps ?inner)"
-          by simp
-        then show ?thesis
-        proof -
-          assume eq_last: "steps pr' ! k = last (steps ?inner)"
-          have "last (steps ?inner) \<in> set (steps ?inner)"
-            using inner_nz by (rule last_in_set)
-          then show ?thesis
-            by (simp only: eq_last)
-        qed
-      qed
-
-      have take_suc_in_steps: "set (take (Suc k) (steps pr')) \<subseteq> set (steps (?acc (Suc k)))"
-      proof -
-        have "take (Suc k) (steps pr') = take k (steps pr') @ [steps pr' ! k]"
-          using k_lt by (simp add: take_Suc_conv_app_nth)
-        then have "set (take (Suc k) (steps pr')) = insert (steps pr' ! k) (set (take k (steps pr')))"
-          by simp
-        moreover have "steps pr' ! k \<in> set (steps (?acc (Suc k)))"
-          using new_eq step_in_inner_steps by simp
-        moreover have "set (take k (steps pr')) \<subseteq> set (steps (?acc (Suc k)))"
-          using take_k_in_steps new_eq by auto
-        ultimately show ?thesis by auto
-      qed
-
-      have valid_suc: "valid_proof F (?acc (Suc k))"
-      proof (cases "k = 0")
-        case True
-        then show ?thesis
-          using new_eq assms(2) inner_valid by simp
-      next
-        case False
-        then have acc_valid: "valid_proof F (?acc k)"
-          using ih by auto
-        have fsys: "frege_system F"
-          using dm1 unfolding de_morgan_frege_def by simp
-        show ?thesis
-          using new_eq acc_valid inner_valid fsys frege_system.combining_valid_proofs by blast
-      qed
-      have thesis_suc: "thesis (?acc (Suc k)) = steps pr' ! k"
-        using new_eq inner_th concl_step by simp
-
-      show ?case
-        using assm_suc take_suc_in_steps valid_suc thesis_suc by auto
-    qed
-  qed
-
-  have final_inv:
-    "assumptions (?acc ?n) = {} \<and>
-     set (take ?n (steps pr')) \<subseteq> set (steps (?acc ?n)) \<and>
-     (?n = 0 \<or> (valid_proof F (?acc ?n) \<and> thesis (?acc ?n) = steps pr' ! (?n - 1)))"
-    using prefix_inv[rule_format, of ?n] by simp
-  have n_nz: "?n \<noteq> 0"
-    using assms(1) unfolding valid_proof_def by simp
-  have final_valid: "valid_proof F (?acc ?n)"
-    using final_inv n_nz by auto
-  have final_assm: "assumptions (?acc ?n) = {}"
-    using final_inv by auto
-  have final_th0: "thesis (?acc ?n) = steps pr' ! (?n - 1)"
-    using final_inv n_nz by auto
-  have final_th: "thesis (?acc ?n) = thesis pr'"
-  proof -
-    have "thesis pr' = last (steps pr')"
-      using assms(1) unfolding valid_proof_def by simp
-    moreover have "last (steps pr') = steps pr' ! (?n - 1)"
-      using n_nz by (simp add: last_conv_nth)
-    ultimately show ?thesis
-      using final_th0 by simp
-  qed
-
-  have pr_eq: "pr = ?acc ?n"
-    using assms(3) unfolding sim_right_def by simp
-  show ?thesis
-    using pr_eq final_valid final_th final_assm by auto
-qed
-
-lemma r_t_t_bound:
-  shows "len_formula (rule_to_taut r) \<le> 
-         len_formula (concl r) + 3 * sum_list (map len_formula (prems r))"
-proof (induction "prems r" arbitrary: r)
-  case Nil
-  hence "r = \<lparr>prems = [], concl = concl r\<rparr>" by simp
-  hence "rule_to_taut r = concl r" using rule_to_taut.simps by metis
-  thus ?case by auto
-next
-  case (Cons x xs)
-  let ?sub_r = "\<lparr>prems = xs, concl = concl r\<rparr>"
-  have "r = \<lparr>prems = x # xs, concl = concl r\<rparr>" using Cons by simp
-  hence "rule_to_taut r = Conn Or [Conn Not [x], rule_to_taut ?sub_r]" 
-    using rule_to_taut.simps(2)[of x xs] by metis
-  hence "len_formula (rule_to_taut r) = 1 + 
-                                        len_formula (Conn Not [x]) + 
-                                        len_formula (rule_to_taut ?sub_r)"
-    by simp
-  also have "... \<le> 2 + len_formula x + len_formula (rule_to_taut ?sub_r)"
-    by simp
-  also have "... \<le> 2 + len_formula x + len_formula (concl r) + 3 * sum_list (map len_formula xs)"
-    using Cons.hyps(1)[of ?sub_r] by simp
-  also have "... \<le> 3 * len_formula x + len_formula (concl r) + 3 * sum_list (map len_formula xs)"
-    using len_formula_positive by auto
-  finally have "len_formula (rule_to_taut r) \<le> 
-                len_formula (concl r) + 3 * sum_list (map len_formula (x # xs))"
-    by simp
-  thus ?case using Cons.hyps(2) by simp
-qed
-
-lemma subs_rule_bound_by_proof:
-  assumes "r \<in> rules F'"
-      and "derived_with i pr r s"
-      and "rule_restricted_sub r s"
-      and "c = Max ((\<lambda> r. length (prems r)) ` rules F') + 1"
-  shows "len_formula (rule_to_taut (sub_rule s r)) \<le> 3 * c * len_proof pr"
-proof -
-  have dwith:
-    "i < length (steps pr)"
-    "concl (sub_rule s r) = steps pr ! i"
-    "\<forall>f1 \<in> set (prems (sub_rule s r)). \<exists>f2 \<in> set (take i (steps pr)). f1 = f2"
-    using assms(2) unfolding derived_with_def by (simp_all add: Let_def)
-  have concl_bound:
-    "len_formula (concl (sub_rule s r)) \<le> len_proof pr"
-  proof -
-    have "concl (sub_rule s r) \<in> set (steps pr)"
-      using dwith(1,2) by (metis in_set_conv_nth)
-    then show ?thesis
-      using spec[OF step_le_proof, of pr] by blast
-  qed
-  have prem_bound:
-    "sum_list (map len_formula (prems (sub_rule s r))) \<le> length (prems (sub_rule s r)) * len_proof pr"
-  proof -
-    have aux:
-      "sum_list (map len_formula xs) \<le> length xs * len_proof pr"
-      if "\<forall>x \<in> set xs. len_formula x \<le> len_proof pr"
-      for xs :: "dformula list"
-      using that
-    proof (induction xs)
-      case Nil
-      then show ?case by simp
-    next
-      case (Cons x xs)
-      have x_bound: "len_formula x \<le> len_proof pr"
-        using Cons.prems by simp
-      have tail_bound: "sum_list (map len_formula xs) \<le> length xs * len_proof pr"
-        using Cons.IH Cons.prems by simp
-      have "sum_list (map len_formula (x # xs)) = len_formula x + sum_list (map len_formula xs)"
-        by simp
-      also have "... \<le> len_proof pr + length xs * len_proof pr"
-        using x_bound tail_bound by simp
-      also have "... = length (x # xs) * len_proof pr"
-        by simp
-      finally show ?case .
-    qed
-    have "\<forall>x \<in> set (prems (sub_rule s r)). len_formula x \<le> len_proof pr"
-    proof
-      fix x
-      assume x_in: "x \<in> set (prems (sub_rule s r))"
-      then obtain f2 where f2_in: "f2 \<in> set (take i (steps pr))" and x_eq: "x = f2"
-        using dwith(3) by blast
-      have "x \<in> set (steps pr)"
-        using f2_in x_eq by (meson in_set_takeD set_take_subset)
-      then show "len_formula x \<le> len_proof pr"
-        using spec[OF step_le_proof, of pr] by blast
-    qed
-    then show ?thesis
-      using aux[of "prems (sub_rule s r)"] by simp
-  qed
-  have r_bound:
-    "len_formula (rule_to_taut (sub_rule s r))
-     \<le> len_formula (concl (sub_rule s r)) + 3 * sum_list (map len_formula (prems (sub_rule s r)))"
-    using r_t_t_bound[of "sub_rule s r"] .
-  have len_prems_max: "length (prems r) \<le> Max ((\<lambda>r. length (prems r)) ` rules F')"
-  proof -
-    have fin_rules: "finite (rules F')"
-      using dm2 unfolding de_morgan_frege_def by (simp add: frege_system.finite)
-    have fin_image: "finite ((\<lambda>r. length (prems r)) ` rules F')"
-      using fin_rules by simp
-    have ne_image: "((\<lambda>r. length (prems r)) ` rules F') \<noteq> {}"
-      using assms(1) by auto
-    have len_in: "length (prems r) \<in> ((\<lambda>r. length (prems r)) ` rules F')"
-      using assms(1) by blast
-    have "length (prems r) \<le> Max ((\<lambda>r. length (prems r)) ` rules F')"
-      using Max_ge[OF fin_image len_in] ne_image by simp
-    then show ?thesis .
-  qed
-  have len_prems_bound: "length (prems r) \<le> c"
-  proof -
-    show ?thesis
-      using len_prems_max assms(4) by simp
-  qed
-  have "len_formula (rule_to_taut (sub_rule s r))
-        \<le> len_proof pr + 3 * (length (prems (sub_rule s r)) * len_proof pr)"
-    using r_bound concl_bound prem_bound by simp
-  also have "... = (1 + 3 * length (prems r)) * len_proof pr"
-    by simp
-  also have "... \<le> (3 * c) * len_proof pr"
-  proof -
-    have c_ge_1: "1 \<le> c"
-      using assms(4) by simp
-    have len_prems_bound': "length (prems r) + 1 \<le> c"
-      using len_prems_max assms(4) by simp
-    have coeff_bound: "1 + 3 * length (prems r) \<le> 3 * c"
-      using len_prems_bound' c_ge_1 by arith
-    show ?thesis
-    proof -
-      have lhs_eq:
-        "sum_list (map len_formula (steps pr)) + 3 * length (prems r) * sum_list (map len_formula (steps pr))
-         = (1 + 3 * length (prems r)) * sum_list (map len_formula (steps pr))"
-        by (simp add: algebra_simps)
-      have rhs_bound:
-        "(1 + 3 * length (prems r)) * sum_list (map len_formula (steps pr))
-         \<le> (3 * c) * sum_list (map len_formula (steps pr))"
-        using mult_right_mono[OF coeff_bound, of "sum_list (map len_formula (steps pr))"] by simp
-      show ?thesis
-        unfolding lhs_eq using rhs_bound by simp
-    qed
-  qed
-  finally show ?thesis by simp
-qed
-
-lemma poly_mono_nat:
-  fixes p :: "nat poly"
-  shows "x \<le> y \<Longrightarrow> poly p x \<le> poly p y"
-proof (induction p)
-  case 0
-  thus ?case by simp
-next
-  case (pCons a p)
-  hence "x * poly p x \<le> y * poly p y"
-    using mult_le_mono by presburger
-  thus ?case by simp
-qed
-
-
-lemma first_step_is_bound_by_proof: 
-  shows "\<exists> g :: (drule \<Rightarrow> nat poly). \<forall> rule \<in> rules F'. \<forall>  pr i sub. 
-            derived_with i pr rule sub \<and> rule_restricted_sub rule sub \<and> valid_proof F' pr \<longrightarrow> 
-            len_proof (first_step rule sub) \<le> poly (g rule) (len_proof pr)"
-proof -
-  let ?c = "Max ((\<lambda>r. card (var_set_rule r)) ` rules F') + 1"
-  obtain g0 :: "drule \<Rightarrow> nat poly" where
-    g0_def: "\<forall>rule \<in> rules F'. \<forall>sub.
-      rule_restricted_sub rule sub \<longrightarrow>
-      len_proof (first_step rule sub) \<le> poly (g0 rule) (len_sub (var_set_rule rule) sub)"
-    using first_step_is_bound by blast
-  let ?g = "\<lambda>rule. pcompose (g0 rule) [:0, ?c:]"
-  have bound_per_rule:
-    "\<forall>rule \<in> rules F'. \<forall>pr i sub.
-      derived_with i pr rule sub \<and> rule_restricted_sub rule sub \<and> valid_proof F' pr \<longrightarrow>
-      len_proof (first_step rule sub) \<le> poly (?g rule) (len_proof pr)"
-  proof (intro ballI allI impI)
-    fix rule pr i sub
-    assume r_in: "rule \<in> rules F'"
-    assume assm: "derived_with i pr rule sub \<and> rule_restricted_sub rule sub \<and> valid_proof F' pr"
-    have dwith: "derived_with i pr rule sub"
-      using assm by simp
-    have rsub: "rule_restricted_sub rule sub"
-      using assm by simp
-    have valid_pr: "valid_proof F' pr"
-      using assm by simp
-    have len_sub_bound: "len_sub (var_set_rule rule) sub \<le> ?c * len_proof pr"
-      using de_morgan_frege.len_sub_bound_by_proof[OF dm2 r_in dwith rsub, of ?c] valid_pr by simp
-    have first_step_bound:
-      "len_proof (first_step rule sub) \<le> poly (g0 rule) (len_sub (var_set_rule rule) sub)"
-      using g0_def r_in rsub by blast
-    have mono_poly:
-      "poly (g0 rule) (len_sub (var_set_rule rule) sub) \<le> poly (g0 rule) (?c * len_proof pr)"
-      using len_sub_bound by (rule poly_mono_nat)
-    have final_poly: "poly (g0 rule) (?c * len_proof pr) = poly (?g rule) (len_proof pr)"
-    proof -
-      have "poly (?g rule) (len_proof pr) = poly (g0 rule) (len_proof pr * ?c)"
-        by (simp add: poly_pcompose algebra_simps)
-      then show ?thesis
-        by (simp add: mult.commute)
-    qed
-    show "len_proof (first_step rule sub) \<le> poly (?g rule) (len_proof pr)"
-      using first_step_bound mono_poly final_poly by arith
-  qed
-  show ?thesis
-    by (intro exI[of _ ?g]) (use bound_per_rule in blast)
-qed
-
-lemma sum_polynomial:
-  fixes S :: "nat poly set"
-  assumes "finite S"
-      and "p = \<Sum> S"
-    shows "\<forall> p' \<in> S. \<forall> n :: nat. poly p n \<ge> poly p' n"
-  by (metis assms(1,2) bot_nat_0.extremum poly_sum sum_nonneg_leq_bound)
-
-lemma first_step_single_bound:
-  shows "\<exists> g :: nat poly. \<forall> rule \<in> rules F'. \<forall>  pr i sub. 
-            derived_with i pr rule sub \<and> rule_restricted_sub rule sub \<and> valid_proof F' pr \<longrightarrow> 
-            len_proof (first_step rule sub) \<le> poly g (len_proof pr)"
-proof (rule exI)
-  let ?gs = "SOME g. \<forall> rule \<in> rules F'. \<forall>  pr i sub. 
-           derived_with i pr rule sub \<and> rule_restricted_sub rule sub \<and> valid_proof F' pr \<longrightarrow> 
-           len_proof (first_step rule sub) \<le> poly (g rule) (len_proof pr)"
-
-  let ?S = "?gs ` (rules F')"
-  have "finite ?S" using dm2 de_morgan_frege_def frege_system_def by auto
-  let ?g = "\<Sum> ?S"
-  show "\<forall>rule\<in>rules F'. \<forall>pr i sub.
-          derived_with i pr rule sub \<and> 
-          rule_restricted_sub rule sub \<and>
-          valid_proof F' pr \<longrightarrow>
-          len_proof (first_step rule sub) \<le> poly ?g (len_proof pr)"
-  proof (intro ballI allI impI)
-    fix rule pr i sub
-    assume r_in: "rule \<in> rules F'"
-    assume assm: "derived_with i pr rule sub \<and> rule_restricted_sub rule sub \<and> valid_proof F' pr"
-    have ex_gs:
-      "\<exists>g :: drule \<Rightarrow> nat poly. \<forall>rule \<in> rules F'. \<forall>pr i sub.
-        derived_with i pr rule sub \<and> rule_restricted_sub rule sub \<and> valid_proof F' pr \<longrightarrow>
-        len_proof (first_step rule sub) \<le> poly (g rule) (len_proof pr)"
-      using first_step_is_bound_by_proof by blast
-    have gs_prop:
-      "\<forall>rule \<in> rules F'. \<forall>pr i sub.
-        derived_with i pr rule sub \<and> rule_restricted_sub rule sub \<and> valid_proof F' pr \<longrightarrow>
-        len_proof (first_step rule sub) \<le> poly (?gs rule) (len_proof pr)"
-      by (rule someI_ex[OF ex_gs])
-    have g_in_S: "?gs rule \<in> ?S"
-      using r_in by simp
-    have sum_bound: "\<forall>p' \<in> ?S. \<forall>n::nat. poly ?g n \<ge> poly p' n"
-      using sum_polynomial[OF \<open>finite ?S\<close>, of ?g] by simp
-    have poly_bound: "poly ?g (len_proof pr) \<ge> poly (?gs rule) (len_proof pr)"
-      using sum_bound g_in_S by blast
-    have step_bound: "len_proof (first_step rule sub) \<le> poly (?gs rule) (len_proof pr)"
-      using gs_prop r_in assm by blast
-    show "len_proof (first_step rule sub) \<le> poly ?g (len_proof pr)"
-      using step_bound poly_bound by arith
-  qed
-qed
-
-lemma second_step_bound:
-  shows "\<exists> g :: nat poly. \<forall> rule \<in> rules F'. \<forall>  pr i sub. 
-            derived_with i pr rule sub \<and> rule_restricted_sub rule sub \<and> valid_proof F' pr \<longrightarrow> 
-            len_proof (second_step (sub_rule sub rule)) \<le> poly g (len_proof pr)"
-proof (rule exI)
-  let ?c = "Max ((\<lambda>r. length (prems r)) ` rules F') + 1"
-  let ?g = "[:0, 0, (3 * ?c)^2:]"
-  show "\<forall>rule\<in>rules F'. \<forall>pr i sub.
-          derived_with i pr rule sub \<and>
-          rule_restricted_sub rule sub \<and> valid_proof F' pr \<longrightarrow>
-          len_proof (second_step (sub_rule sub rule)) \<le> poly ?g (len_proof pr)"
-  proof (intro ballI allI impI)
-    fix rule pr i sub
-    assume r_in: "rule \<in> rules F'"
-    assume assm: "derived_with i pr rule sub \<and> rule_restricted_sub rule sub \<and> valid_proof F' pr"
-    let ?rsub = "sub_rule sub rule"
-    have dwith: "derived_with i pr rule sub"
-      using assm by simp
-    have rsub: "rule_restricted_sub rule sub"
-      using assm by simp
-    obtain p where peel_res: "peel (rule_to_taut ?rsub) (concl ?rsub) = Some p"
-      using r_t_t_peelable[of ?rsub] by blast
-    have step_eq: "second_step ?rsub = p"
-      using peel_res by simp
-    have peel_b: "len_proof p \<le> (len_formula (rule_to_taut ?rsub))^2"
-      using peel_bound[OF peel_res] .
-    have taut_b: "len_formula (rule_to_taut ?rsub) \<le> 3 * ?c * len_proof pr"
-      using subs_rule_bound_by_proof[OF r_in dwith rsub, of ?c] by simp
-    have proof_b: "len_proof p \<le> (3 * ?c * len_proof pr)^2"
-    proof -
-      have nonneg: "0 \<le> len_formula (rule_to_taut ?rsub)"
-        by simp
-      have "(len_formula (rule_to_taut ?rsub))^2 \<le> (3 * ?c * len_proof pr)^2"
-        using taut_b nonneg by (rule power_mono)
-      then show ?thesis
-        using peel_b by linarith
-    qed
-    have poly_eq: "poly ?g (len_proof pr) = (3 * ?c * len_proof pr)^2"
-      by (simp add: power2_eq_square algebra_simps)
-    show "len_proof (second_step (sub_rule sub rule)) \<le> poly ?g (len_proof pr)"
-      using step_eq proof_b poly_eq by simp
-  qed
-qed
-
-
-lemma sim_right_step_bound:
-  shows "\<exists> bound. \<forall> pr i acc. i \<ge> 0 \<and> i < length (steps pr) \<and> valid_proof F' pr \<longrightarrow>
-            len_proof (sim_right_step pr i acc) \<le> poly bound (len_proof pr) + len_proof acc"
-proof -
-  obtain g1 :: "nat poly" where g1_prop:
-    "\<forall>rule\<in>rules F'. \<forall>pr i sub.
-      derived_with i pr rule sub \<and> rule_restricted_sub rule sub \<and> valid_proof F' pr \<longrightarrow>
-      len_proof (first_step rule sub) \<le> poly g1 (len_proof pr)"
-    using first_step_single_bound by blast
-  obtain g2 :: "nat poly" where g2_prop:
-    "\<forall>rule\<in>rules F'. \<forall>pr i sub.
-      derived_with i pr rule sub \<and> rule_restricted_sub rule sub \<and> valid_proof F' pr \<longrightarrow>
-      len_proof (second_step (sub_rule sub rule)) \<le> poly g2 (len_proof pr)"
-    using second_step_bound by blast
-  let ?bound = "[:0, 1:] + g1 + g2"
-  show ?thesis
-  proof (rule exI[of _ ?bound], intro allI impI)
-    fix pr i acc
-    assume assm: "i \<ge> 0 \<and> i < length (steps pr) \<and> valid_proof F' pr"
-    have i_lt: "i < length (steps pr)"
-      using assm by simp
-    have pr_valid: "valid_proof F' pr"
-      using assm by simp
-    let ?step = "steps pr ! i"
-
-    have sub_formula_agree:
-      "sub_formula s1 f = sub_formula s2 f"
-      if "\<forall>v \<in> var_set_form f. s1 v = s2 v"
-      for s1 s2 :: "string \<Rightarrow> dformula" and f
-      using that
-    proof (induction f)
-      case (Atom x)
-      then show ?case by simp
-    next
-      case (Conn c fs)
-      then show ?case by simp
-    qed
-
-    have sub_rule_agree:
-      "sub_rule s1 r = sub_rule s2 r"
-      if "\<forall>v \<in> var_set_rule r. s1 v = s2 v"
-      for s1 s2 :: "string \<Rightarrow> dformula" and r
-      using that
-      by (cases r) (auto intro: sub_formula_agree)
-
-    have choose_rule_sub_props:
-      "\<not> ?step \<in> assumptions pr \<Longrightarrow>
-       fst (choose_rule_sub F' i pr) \<in> rules F' \<and>
-       derived_with i pr (fst (choose_rule_sub F' i pr)) (snd (choose_rule_sub F' i pr)) \<and>
-       rule_restricted_sub (fst (choose_rule_sub F' i pr)) (snd (choose_rule_sub F' i pr))"
-    proof -
-      assume step_notin: "?step \<notin> assumptions pr"
-      have step_der:
-        "derived (rules F') (take i (steps pr)) ?step"
-        using pr_valid i_lt step_notin
-        unfolding valid_proof_def by auto
-      then obtain r s where r_in: "r \<in> rules F'"
-        and d_concl: "concl (sub_rule s r) = ?step"
-        and d_prems:
-          "\<forall>f1\<in>set (prems (sub_rule s r)). \<exists>f2\<in>set (take i (steps pr)). f1 = f2"
-        unfolding derived_def by auto
-      have dwith: "derived_with i pr r s"
-        using i_lt d_concl d_prems
-        unfolding derived_with_def by simp
-      define s' where "s' = (\<lambda>v. if v \<in> var_set_rule r then s v else Atom v)"
-      have sr_eq: "sub_rule s' r = sub_rule s r"
-        unfolding s'_def
-        by (rule sub_rule_agree) auto
-      have dwith': "derived_with i pr r s'"
-        using dwith unfolding derived_with_def sr_eq by simp
-      have rsub': "rule_restricted_sub r s'"
-        unfolding rule_restricted_sub_def s'_def by simp
-      let ?P = "\<lambda>rs :: drule \<times> (string \<Rightarrow> dformula).
-        case rs of (r, s) \<Rightarrow> r \<in> rules F' \<and> derived_with i pr r s \<and> rule_restricted_sub r s"
-      have ex_pair: "\<exists>rs. ?P rs"
-        using r_in dwith' rsub' by force
-      have "?P (SOME rs. ?P rs)"
-        by (rule someI_ex[OF ex_pair])
-      then show "fst (choose_rule_sub F' i pr) \<in> rules F' \<and>
-                 derived_with i pr (fst (choose_rule_sub F' i pr)) (snd (choose_rule_sub F' i pr)) \<and>
-                 rule_restricted_sub (fst (choose_rule_sub F' i pr)) (snd (choose_rule_sub F' i pr))"
-        unfolding choose_rule_sub_def
-        by (cases "SOME rs. ?P rs") auto
-    qed
-
-    show "len_proof (sim_right_step pr i acc) \<le> poly ?bound (len_proof pr) + len_proof acc"
-    proof (cases "?step \<in> assumptions pr")
-      case True
-      have step_in: "?step \<in> set (steps pr)"
-        using i_lt by simp
-      have step_b: "len_formula ?step \<le> len_proof pr"
-        using step_le_proof step_in by blast
-      have "len_proof (sim_right_step pr i acc)
-            = len_proof acc + len_formula ?step"
-        using True i_lt unfolding sim_right_step_def by (simp add: Let_def)
-      also have "\<dots> \<le> len_proof acc + len_proof pr"
-        using step_b by simp
-      also have "\<dots> = len_proof acc + poly [:0, 1:] (len_proof pr)"
-        by simp
-      also have "\<dots> \<le> len_proof acc + poly ?bound (len_proof pr)"
-        by simp
-      finally show ?thesis
-        by (simp add: add.commute add.left_commute add.assoc)
-    next
-      case False
-      have choose_props:
-        "fst (choose_rule_sub F' i pr) \<in> rules F' \<and>
-         derived_with i pr (fst (choose_rule_sub F' i pr)) (snd (choose_rule_sub F' i pr)) \<and>
-         rule_restricted_sub (fst (choose_rule_sub F' i pr)) (snd (choose_rule_sub F' i pr))"
-        using choose_rule_sub_props False by blast
-      let ?rule = "fst (choose_rule_sub F' i pr)"
-      let ?sub = "snd (choose_rule_sub F' i pr)"
-      have r_in: "?rule \<in> rules F'"
-        using choose_props by simp
-      have dwith: "derived_with i pr ?rule ?sub"
-        using choose_props by simp
-      have rsub: "rule_restricted_sub ?rule ?sub"
-        using choose_props by simp
-      have first_b: "len_proof (first_step ?rule ?sub) \<le> poly g1 (len_proof pr)"
-        using g1_prop r_in dwith rsub pr_valid by blast
-      have second_b: "len_proof (second_step (sub_rule ?sub ?rule)) \<le> poly g2 (len_proof pr)"
-        using g2_prop r_in dwith rsub pr_valid by blast
-      have step_eq:
-        "sim_right_step pr i acc
-         = combine_proofs acc
-             (combine_proofs (first_step ?rule ?sub) (second_step (sub_rule ?sub ?rule)))"
-      proof (cases "choose_rule_sub F' i pr")
-        case (Pair r s)
-        then show ?thesis
-          using False i_lt by (simp add: sim_right_step_def Let_def)
-      qed
-      have "len_proof (sim_right_step pr i acc)
-            = len_proof acc + len_proof (first_step ?rule ?sub)
-              + len_proof (second_step (sub_rule ?sub ?rule))"
-        using step_eq by (simp add: add.assoc)
-      also have "\<dots> \<le> len_proof acc + poly g1 (len_proof pr) + poly g2 (len_proof pr)"
-        using first_b second_b by simp
-      also have "\<dots> \<le> len_proof acc + poly ?bound (len_proof pr)"
-        by simp
-      finally show ?thesis
-        by (simp add: add.assoc add.commute add.left_commute)
-    qed
-  qed
-qed
-
-lemma sim_right_bound:
-  assumes "valid_proof F' pr \<and> assumptions pr = {}"
-  shows "\<exists> bound. len_proof (sim_right pr (thesis pr)) \<le> poly bound (len_proof pr)"
-proof -
-  obtain g :: "nat poly" where g_prop:
-    "\<forall>pr i acc. i \<ge> 0 \<and> i < length (steps pr) \<and> valid_proof F' pr \<longrightarrow>
-      len_proof (sim_right_step pr i acc) \<le> poly g (len_proof pr) + len_proof acc"
-    using sim_right_step_bound by blast
-  let ?acc = "\<lambda>k. fold (sim_right_step pr) [0..<k] \<lparr>assumptions = assumptions pr, thesis = thesis pr, steps = []\<rparr>"
-  have pr_valid: "valid_proof F' pr"
-    using assms by simp
-  have steps_bound: "length (steps pr) \<le> len_proof pr"
-  proof -
-    have ones_le_list:
-      "sum_list (replicate (length fs) 1) \<le> sum_list (map len_formula fs)" for fs :: "dformula list"
-    proof (induction fs)
-      case Nil
-      then show ?case by simp
-    next
-      case (Cons f fs)
-      have "1 + sum_list (replicate (length fs) 1) \<le> len_formula f + sum_list (map len_formula fs)"
-        using Cons.IH len_formula_positive[of f] by simp
-      then show ?case by simp
-    qed
-    have ones_le:
-      "sum_list (replicate (length (steps pr)) 1) \<le> sum_list (map len_formula (steps pr))"
-      using ones_le_list[of "steps pr"] .
-    have ones_eq_list: "sum_list (replicate (length fs) 1) = length fs" for fs :: "dformula list"
-    proof (induction fs)
-      case Nil
-      then show ?case by simp
-    next
-      case (Cons f fs)
-      then show ?case by simp
-    qed
-    have ones_eq: "sum_list (replicate (length (steps pr)) 1) = length (steps pr)"
-      using ones_eq_list[of "steps pr"] .
-    then have "length (steps pr) \<le> sum_list (map len_formula (steps pr))"
-      using ones_le by simp
-    then show ?thesis by simp
-  qed
-  have fold_bound:
-    "\<forall>k\<le>length (steps pr). len_proof (?acc k) \<le> k * poly g (len_proof pr)"
-  proof (intro allI impI)
-    fix k
-    assume k_le: "k \<le> length (steps pr)"
-    show "len_proof (?acc k) \<le> k * poly g (len_proof pr)"
-      using k_le
-    proof (induction k)
-      case 0
-      then show ?case by simp
-    next
-      case (Suc k)
-      have k_le_steps: "k < length (steps pr)"
-        using Suc.prems by simp
-      have ih: "len_proof (?acc k) \<le> k * poly g (len_proof pr)"
-        using Suc.IH Suc.prems by simp
-      have step_b:
-        "len_proof (sim_right_step pr k (?acc k)) \<le> poly g (len_proof pr) + len_proof (?acc k)"
-        using g_prop k_le_steps pr_valid by simp
-      have "?acc (Suc k) = sim_right_step pr k (?acc k)"
-        by simp
-      then have "len_proof (?acc (Suc k)) \<le> poly g (len_proof pr) + len_proof (?acc k)"
-        using step_b by simp
-      also have "\<dots> \<le> poly g (len_proof pr) + k * poly g (len_proof pr)"
-        using ih by simp
-      also have "\<dots> = Suc k * poly g (len_proof pr)"
-        by simp
-      finally show ?case .
-    qed
-  qed
-  let ?bound = "[:0, 1:] * g"
-  have final_fold:
-    "len_proof (sim_right pr (thesis pr)) \<le> length (steps pr) * poly g (len_proof pr)"
-    unfolding sim_right_def using fold_bound by simp
-  also have "\<dots> \<le> len_proof pr * poly g (len_proof pr)"
-    using steps_bound by simp
-  also have "\<dots> = poly ?bound (len_proof pr)"
-    by simp
-  finally show ?thesis
-    by (rule exI[of _ ?bound])
-qed
-
-lemma simulation_de_morgan_right:
-  shows "simulates F' F"
-proof -
-  obtain g :: "nat poly" where g_prop:
-    "\<forall>pr i acc. i \<ge> 0 \<and> i < length (steps pr) \<and> valid_proof F' pr \<longrightarrow>
-      len_proof (sim_right_step pr i acc) \<le> poly g (len_proof pr) + len_proof acc"
-    using sim_right_step_bound by blast
-  let ?f = "\<lambda>w \<tau>. sim_right w (thesis w)"
-  let ?g = "\<lambda>\<tau>. \<tau>"
-  let ?p = "[:0, 1:]"
-  let ?q = "[:0, 1:] * g"
-  have sim_case:
-    "(thesis w = ?g \<tau> \<and> valid_proof F' w \<and> assumptions w = {}) \<longrightarrow>
-      valid_proof F (?f w \<tau>) \<and> thesis (?f w \<tau>) = \<tau> \<and> assumptions (?f w \<tau>) = {} \<and>
-      len_formula (?g \<tau>) \<le> poly ?p (len_formula \<tau>) \<and>
-      len_proof (?f w \<tau>) \<le> poly ?q (len_proof w)" for w \<tau>
-  proof
-    assume assm: "thesis w = ?g \<tau> \<and> valid_proof F' w \<and> assumptions w = {}"
-    have th_eq: "thesis w = \<tau>"
-      using assm by simp
-    have w_valid: "valid_proof F' w"
-      using assm by simp
-    have w_assm: "assumptions w = {}"
-      using assm by simp
-
-    have pr_props:
-      "valid_proof F (?f w \<tau>) \<and> thesis (?f w \<tau>) = thesis w \<and> assumptions (?f w \<tau>) = {}"
-      using sim_right_proves[of w "sim_right w (thesis w)"] w_valid w_assm by simp
-    have local_bound:
-      "\<exists>bound. len_proof (sim_right w (thesis w)) \<le> poly bound (len_proof w)"
-      using sim_right_bound[of w] w_valid w_assm by simp
-
-    let ?acc = "\<lambda>k. fold (sim_right_step w) [0..<k]
-      \<lparr>assumptions = assumptions w, thesis = thesis w, steps = []\<rparr>"
-    have steps_bound: "length (steps w) \<le> len_proof w"
-    proof -
-      have ones_le_list:
-        "sum_list (replicate (length fs) 1) \<le> sum_list (map len_formula fs)" for fs :: "dformula list"
-      proof (induction fs)
-        case Nil
-        then show ?case by simp
-      next
-        case (Cons f fs)
-        have "1 + sum_list (replicate (length fs) 1) \<le> len_formula f + sum_list (map len_formula fs)"
-          using Cons.IH len_formula_positive[of f] by simp
-        then show ?case by simp
-      qed
-      have ones_le:
-        "sum_list (replicate (length (steps w)) 1) \<le> sum_list (map len_formula (steps w))"
-        using ones_le_list[of "steps w"] .
-      have ones_eq_list: "sum_list (replicate (length fs) 1) = length fs" for fs :: "dformula list"
-      proof (induction fs)
-        case Nil
-        then show ?case by simp
-      next
-        case (Cons f fs)
-        then show ?case by simp
-      qed
-      have ones_eq: "sum_list (replicate (length (steps w)) 1) = length (steps w)"
-        using ones_eq_list[of "steps w"] .
-      then have "length (steps w) \<le> sum_list (map len_formula (steps w))"
-        using ones_le by simp
-      then show ?thesis by simp
-    qed
-    have fold_bound:
-      "\<forall>k\<le>length (steps w). len_proof (?acc k) \<le> k * poly g (len_proof w)"
-    proof (intro allI impI)
-      fix k
-      assume k_le: "k \<le> length (steps w)"
-      show "len_proof (?acc k) \<le> k * poly g (len_proof w)"
-        using k_le
-      proof (induction k)
-        case 0
-        then show ?case by simp
-      next
-        case (Suc k)
-        have k_lt: "k < length (steps w)"
-          using Suc.prems by simp
-        have ih: "len_proof (?acc k) \<le> k * poly g (len_proof w)"
-          using Suc.IH Suc.prems by simp
-        have step_b:
-          "len_proof (sim_right_step w k (?acc k)) \<le> poly g (len_proof w) + len_proof (?acc k)"
-          using g_prop k_lt w_valid by simp
-        have "?acc (Suc k) = sim_right_step w k (?acc k)"
-          by simp
-        then have "len_proof (?acc (Suc k)) \<le> poly g (len_proof w) + len_proof (?acc k)"
-          using step_b by simp
-        also have "\<dots> \<le> poly g (len_proof w) + k * poly g (len_proof w)"
-          using ih by simp
-        also have "\<dots> = Suc k * poly g (len_proof w)"
-          by simp
-        finally show ?case .
-      qed
-    qed
-    have global_bound:
-      "len_proof (?f w \<tau>) \<le> poly ?q (len_proof w)"
-    proof -
-      have "len_proof (sim_right w (thesis w)) \<le> length (steps w) * poly g (len_proof w)"
-        unfolding sim_right_def using fold_bound by simp
-      also have "\<dots> \<le> len_proof w * poly g (len_proof w)"
-        using steps_bound by simp
-      also have "\<dots> = poly ?q (len_proof w)"
-        by simp
-      finally show ?thesis by simp
-    qed
-
-    show "valid_proof F (?f w \<tau>) \<and> thesis (?f w \<tau>) = \<tau> \<and> assumptions (?f w \<tau>) = {} \<and>
-      len_formula (?g \<tau>) \<le> poly ?p (len_formula \<tau>) \<and>
-      len_proof (?f w \<tau>) \<le> poly ?q (len_proof w)"
-    proof -
-      have valid_f: "valid_proof F (?f w \<tau>)"
-        using pr_props by simp
-      have thesis_f: "thesis (?f w \<tau>) = \<tau>"
-        using pr_props th_eq by simp
-      have assm_f: "assumptions (?f w \<tau>) = {}"
-        using pr_props by simp
-      have len_g: "len_formula (?g \<tau>) \<le> poly ?p (len_formula \<tau>)"
-        by simp
-      show ?thesis
-      proof (intro conjI)
-        show "valid_proof F (?f w \<tau>)"
-          using valid_f .
-        show "thesis (?f w \<tau>) = \<tau>"
-          using thesis_f .
-        show "assumptions (?f w \<tau>) = {}"
-          using assm_f .
-        show "len_formula (?g \<tau>) \<le> poly ?p (len_formula \<tau>)"
-          using len_g .
-        show "len_proof (?f w \<tau>) \<le> poly ?q (len_proof w)"
-          using global_bound .
-      qed
-    qed
-  qed
-  show ?thesis
-    unfolding simulates_def
-  proof (rule exI[of _ ?f], rule exI[of _ ?g], rule exI[of _ ?p], rule exI[of _ ?q], intro allI)
-    fix w \<tau>
-    show "thesis w = ?g \<tau> \<and> valid_proof F' w \<and> assumptions w = {} \<longrightarrow>
-      valid_proof F (?f w \<tau>) \<and> thesis (?f w \<tau>) = \<tau> \<and> assumptions (?f w \<tau>) = {} \<and>
-      len_formula (?g \<tau>) \<le> poly ?p (len_formula \<tau>) \<and>
-      len_proof (?f w \<tau>) \<le> poly ?q (len_proof w)"
-      using sim_case[of w \<tau>] .
-  qed
-qed
-
-
-lemma fixed_proofs_rules_F:
-  shows "\<forall> rule \<in> rules F. \<exists> pr. 
-          valid_proof F' pr \<and> 
-          assumptions pr = set (prems rule) \<and> 
-          thesis pr = concl rule"
-  by (meson de_morgan_frege_def dm1 dm2 proof_exists_for_rule)
-
-lemma rule_proof_fun_F_exists: "\<exists> f :: drule \<Rightarrow> dproof. \<forall> rule \<in> rules F.
-          valid_proof F' (f rule) \<and> 
-          assumptions (f rule) = set (prems rule) \<and> 
-          thesis (f rule) = concl rule"
-  by (meson fixed_proofs_rules_F)
-
-definition rule_proof_fun_F where
-  "rule_proof_fun_F = (SOME f. \<forall> rule \<in> rules F.
-          valid_proof F' (f rule) \<and> 
-          assumptions (f rule) = set (prems rule) \<and> 
-          thesis (f rule) = concl rule)"
-
-fun step_F :: "drule \<Rightarrow> (string \<Rightarrow> dformula) \<Rightarrow> dproof" where
-  "step_F rule sub = sub_proof sub (rule_proof_fun_F rule)"
-
-lemma step_F_proves:
-  assumes "r \<in> rules F"
-  shows "valid_proof F' (step_F r s) \<and>
-         assumptions (step_F r s) = set (prems (sub_rule s r)) \<and>
-         thesis (step_F r s) = concl (sub_rule s r)"
-proof -
-  have ex_fun:
-    "\<exists>f :: drule \<Rightarrow> dproof. \<forall>rule \<in> rules F.
-      valid_proof F' (f rule) \<and> assumptions (f rule) = set (prems rule) \<and> thesis (f rule) = concl rule"
-    using rule_proof_fun_F_exists .
-  have fun_prop:
-    "\<forall>rule \<in> rules F.
-      valid_proof F' (rule_proof_fun_F rule) \<and>
-      assumptions (rule_proof_fun_F rule) = set (prems rule) \<and>
-      thesis (rule_proof_fun_F rule) = concl rule"
-    unfolding rule_proof_fun_F_def by (rule someI_ex[OF ex_fun])
-  then have base:
-    "valid_proof F' (rule_proof_fun_F r) \<and>
-     assumptions (rule_proof_fun_F r) = set (prems r) \<and>
-     thesis (rule_proof_fun_F r) = concl r"
-    using assms by blast
-  then have base_valid: "valid_proof F' (rule_proof_fun_F r)"
-    and base_assm: "assumptions (rule_proof_fun_F r) = set (prems r)"
-    and base_th: "thesis (rule_proof_fun_F r) = concl r"
-    by auto
-  have fsys: "frege_system F'"
-    using dm2 unfolding de_morgan_frege_def by simp
-  interpret fs: frege_system F'
-    by (rule fsys)
-  have sub_valid: "valid_proof F' (step_F r s)"
-    unfolding step_F.simps using fs.proof_substitution[OF base_valid] .
-  have sub_assm: "assumptions (step_F r s) = set (prems (sub_rule s r))"
-    using base_assm by simp
-  have sub_th: "thesis (step_F r s) = concl (sub_rule s r)"
-    using base_th by simp
-  show ?thesis
-    using sub_valid sub_assm sub_th by simp
-qed
-
-
-definition sim_left_step :: "dproof \<Rightarrow> nat \<Rightarrow> dproof \<Rightarrow> dproof" where
-  "sim_left_step pr i acc =
-    (let step = (steps pr) ! i in
-      if step \<in> assumptions pr then 
-        combine_proofs acc \<lparr>assumptions = {}, thesis = step, steps = [step]\<rparr>
-      else
-        let (r, s) = choose_rule_sub F i pr in
-        let pr = step_F r s
-        in combine_proofs acc pr)"
-
-definition sim_left :: "dproof \<Rightarrow> dformula \<Rightarrow> dproof" where
-  "sim_left pr th =
-     fold (sim_left_step pr)
-       [0..<length (steps pr)]
-       \<lparr>assumptions = assumptions pr,
-        thesis = th,
-        steps = []\<rparr>"
-
-lemma sim_left_step_progress:
+lemma sim_step_progress:
   fixes pr acc :: dproof
   assumes valid_pr: "valid_proof F pr"
       and assm_pr: "assumptions pr = {}"
@@ -2023,10 +391,10 @@ lemma sim_left_step_progress:
       and acc_steps: "set (take k (steps pr)) \<subseteq> set (steps acc)"
       and acc_valid: "k = 0 \<or> valid_proof F' acc"
       and acc0: "k = 0 \<longrightarrow> steps acc = []"
-  shows "assumptions (sim_left_step pr k acc) = {} \<and>
-         valid_proof F' (sim_left_step pr k acc) \<and>
-         thesis (sim_left_step pr k acc) = steps pr ! k \<and>
-         set (take (Suc k) (steps pr)) \<subseteq> set (steps (sim_left_step pr k acc))"
+  shows "assumptions (sim_step pr k acc) = {} \<and>
+         valid_proof F' (sim_step pr k acc) \<and>
+         thesis (sim_step pr k acc) = steps pr ! k \<and>
+         set (take (Suc k) (steps pr)) \<subseteq> set (steps (sim_step pr k acc))"
 proof -
   let ?step = "steps pr ! k"
   have step_not_assm: "?step \<notin> assumptions pr"
@@ -2043,10 +411,10 @@ proof -
   let ?r = "fst (choose_rule_sub F k pr)"
   let ?s = "snd (choose_rule_sub F k pr)"
   have step_props:
-    "valid_proof F' (step_F ?r ?s) \<and>
-     assumptions (step_F ?r ?s) = set (prems (sub_rule ?s ?r)) \<and>
-     thesis (step_F ?r ?s) = concl (sub_rule ?s ?r)"
-    using step_F_proves choose_props by blast
+    "valid_proof F' (step_proof ?r ?s) \<and>
+     assumptions (step_proof ?r ?s) = set (prems (sub_rule ?s ?r)) \<and>
+     thesis (step_proof ?r ?s) = concl (sub_rule ?s ?r)"
+    using step_proof_proves choose_props by blast
   have dchoose: "derived_with k pr ?r ?s"
     using choose_props by simp
   have prems_seen: "set (prems (sub_rule ?s ?r)) \<subseteq> set (steps acc)"
@@ -2058,26 +426,26 @@ proof -
     thus "f \<in> set (steps acc)"
       using acc_steps by blast
   qed
-  have eq: "sim_left_step pr k acc = combine_proofs acc (step_F ?r ?s)"
+  have eq: "sim_step pr k acc = combine_proofs acc (step_proof ?r ?s)"
   proof (cases "choose_rule_sub F k pr")
     case (Pair r s)
     then show ?thesis
-      using step_not_assm k_lt by (simp add: sim_left_step_def Let_def)
+      using step_not_assm k_lt by (simp add: sim_step_def Let_def)
   qed
-  have valid_next: "valid_proof F' (sim_left_step pr k acc)"
+  have valid_next: "valid_proof F' (sim_step pr k acc)"
   proof (cases "k = 0")
     case True
-    have step_valid: "valid_proof F' (step_F ?r ?s)"
+    have step_valid: "valid_proof F' (step_proof ?r ?s)"
       using step_props by blast
     have acc_steps0: "steps acc = []"
       using True acc0 by simp
-    have comb_eq: "combine_proofs acc (step_F ?r ?s) = step_F ?r ?s"
+    have comb_eq: "combine_proofs acc (step_proof ?r ?s) = step_proof ?r ?s"
       using acc_assm acc_steps0 step_props by (cases acc) simp
-    have "sim_left_step pr k acc = combine_proofs acc (step_F ?r ?s)"
+    have "sim_step pr k acc = combine_proofs acc (step_proof ?r ?s)"
       using eq .
-    also have "\<dots> = step_F ?r ?s"
+    also have "\<dots> = step_proof ?r ?s"
       using comb_eq .
-    finally have "sim_left_step pr k acc = step_F ?r ?s" .
+    finally have "sim_step pr k acc = step_proof ?r ?s" .
     then show ?thesis
       using step_valid by simp
   next
@@ -2090,9 +458,9 @@ proof -
       using eq acc_valid' step_props prems_seen fsys frege_system.combining_valid_proofs
       by blast
   qed
-  have assm_next: "assumptions (sim_left_step pr k acc) = {}"
+  have assm_next: "assumptions (sim_step pr k acc) = {}"
     using eq acc_assm step_props prems_seen by simp
-  have steps_next: "set (take (Suc k) (steps pr)) \<subseteq> set (steps (sim_left_step pr k acc))"
+  have steps_next: "set (take (Suc k) (steps pr)) \<subseteq> set (steps (sim_step pr k acc))"
   proof
     fix f
     assume "f \<in> set (take (Suc k) (steps pr))"
@@ -2105,7 +473,7 @@ proof -
       using fi_take i_lt k_lt by simp
     consider "i < k" | "i = k"
       using i_lt by linarith
-    then show "f \<in> set (steps (sim_left_step pr k acc))"
+    then show "f \<in> set (steps (sim_step pr k acc))"
     proof cases
       case 1
       have i_take: "i < length (take k (steps pr))"
@@ -2124,17 +492,17 @@ proof -
       case 2
       have "concl (sub_rule ?s ?r) = steps pr ! k"
         using dchoose unfolding derived_with_def by simp
-      moreover have "thesis (step_F ?r ?s) = concl (sub_rule ?s ?r)"
+      moreover have "thesis (step_proof ?r ?s) = concl (sub_rule ?s ?r)"
         using step_props by blast
-      moreover have "valid_proof F' (step_F ?r ?s)"
+      moreover have "valid_proof F' (step_proof ?r ?s)"
         using step_props by blast
-      then have "thesis (step_F ?r ?s) \<in> set (steps (step_F ?r ?s))"
+      then have "thesis (step_proof ?r ?s) \<in> set (steps (step_proof ?r ?s))"
         unfolding valid_proof_def by (metis last_in_set)
       ultimately show ?thesis
         using 2 fi eq by auto
     qed
   qed
-  have thesis_next: "thesis (sim_left_step pr k acc) = steps pr ! k"
+  have thesis_next: "thesis (sim_step pr k acc) = steps pr ! k"
   proof -
     have "concl (sub_rule ?s ?r) = steps pr ! k"
       using dchoose unfolding derived_with_def by simp
@@ -2144,16 +512,15 @@ proof -
     using assm_next valid_next thesis_next steps_next by simp
 qed
 
-
-lemma sim_left_proves:
+lemma sim_proves:
   fixes pr :: dproof
   assumes "valid_proof F pr"
   and "assumptions pr = {}"
-  and "pr' = sim_left pr (thesis pr)"
+  and "pr' = sim pr (thesis pr)"
 shows "valid_proof F' pr' \<and> thesis pr' = thesis pr \<and> assumptions pr' = {}"
 proof -
   let ?init = "\<lparr>assumptions = assumptions pr, thesis = thesis pr, steps = []\<rparr>"
-  let ?acc = "\<lambda>k. fold (sim_left_step pr) [0..<k] ?init"
+  let ?acc = "\<lambda>k. fold (sim_step pr) [0..<k] ?init"
   let ?n = "length (steps pr)"
 
   have prefix_inv:
@@ -2181,11 +548,11 @@ proof -
       have acc0: "k = 0 \<longrightarrow> steps (?acc k) = []"
         by (cases k) simp_all
       have step_prog:
-        "assumptions (sim_left_step pr k (?acc k)) = {} \<and>
-         valid_proof F' (sim_left_step pr k (?acc k)) \<and>
-         thesis (sim_left_step pr k (?acc k)) = steps pr ! k \<and>
-         set (take (Suc k) (steps pr)) \<subseteq> set (steps (sim_left_step pr k (?acc k)))"
-        using sim_left_step_progress[of pr k "?acc k"] assms k_lt acc0 IH by blast
+        "assumptions (sim_step pr k (?acc k)) = {} \<and>
+         valid_proof F' (sim_step pr k (?acc k)) \<and>
+         thesis (sim_step pr k (?acc k)) = steps pr ! k \<and>
+         set (take (Suc k) (steps pr)) \<subseteq> set (steps (sim_step pr k (?acc k)))"
+        using sim_step_progress[of pr k "?acc k"] assms k_lt acc0 IH by blast
       show ?case
         using step_prog by simp
     qed
@@ -2209,16 +576,16 @@ proof -
     finally show ?thesis .
   qed
   show ?thesis
-    using assms(3) final_assm final_valid final_thesis unfolding sim_left_def by auto
+    using assms(3) final_assm final_valid final_thesis unfolding sim_def by auto
 qed
 
-lemma step_F_bound:
+lemma step_proof_bound:
   shows "\<exists> g :: nat poly. \<forall> rule \<in> rules F. \<forall>  pr i sub. 
             derived_with i pr rule sub \<and> rule_restricted_sub rule sub \<and> valid_proof F pr \<longrightarrow> 
-            len_proof (step_F rule sub) \<le> poly g (len_proof pr)"
+            len_proof (step_proof rule sub) \<le> poly g (len_proof pr)"
 proof -
   let ?c = "Max ((\<lambda>r. card (var_set_rule r)) ` rules F) + 1"
-  let ?S = "(\<lambda>r. ?c * len_proof (rule_proof_fun_F r)) ` rules F"
+  let ?S = "(\<lambda>r. ?c * len_proof (rule_proof_fun r)) ` rules F"
   let ?g = "[:0, Max ?S:]"
   have fin_rules: "finite (rules F)"
     using dm1 unfolding de_morgan_frege_def by (simp add: frege_system.finite)
@@ -2238,48 +605,49 @@ proof -
     have restricted_sub: "\<forall>v. v \<notin> var_set_rule rule \<longrightarrow> sub v = Atom v"
       using rsub unfolding rule_restricted_sub_def by simp
     have step_bound:
-      "len_proof (step_F rule sub)
-       \<le> len_proof (rule_proof_fun_F rule) * len_sub (var_set_rule rule) sub"
-      unfolding step_F.simps
-      using sub_proof_bound[of "var_set_rule rule" sub "rule_proof_fun_F rule"] var_set_rule_finite[of rule] restricted_sub
+      "len_proof (step_proof rule sub)
+       \<le> len_proof (rule_proof_fun rule) * len_sub (var_set_rule rule) sub"
+      unfolding step_proof.simps
+      using sub_proof_bound[of "var_set_rule rule" sub "rule_proof_fun rule"] var_set_rule_finite[of rule] restricted_sub
       by simp
     have step_bound':
-      "len_proof (step_F rule sub)
-       \<le> (?c * len_proof (rule_proof_fun_F rule)) * len_proof pr"
+      "len_proof (step_proof rule sub)
+       \<le> (?c * len_proof (rule_proof_fun rule)) * len_proof pr"
     proof -
-      have coeff_nonneg: "0 \<le> len_proof (rule_proof_fun_F rule)"
+      have coeff_nonneg: "0 \<le> len_proof (rule_proof_fun rule)"
         by simp
       have mult_bound:
-        "len_proof (rule_proof_fun_F rule) * len_sub (var_set_rule rule) sub
-         \<le> len_proof (rule_proof_fun_F rule) * (?c * len_proof pr)"
+        "len_proof (rule_proof_fun rule) * len_sub (var_set_rule rule) sub
+         \<le> len_proof (rule_proof_fun rule) * (?c * len_proof pr)"
         using len_sub_bound coeff_nonneg by (rule mult_left_mono)
-      have "len_proof (step_F rule sub) \<le> len_proof (rule_proof_fun_F rule) * (?c * len_proof pr)"
+      have "len_proof (step_proof rule sub) \<le> len_proof (rule_proof_fun rule) * (?c * len_proof pr)"
         using step_bound mult_bound by linarith
       then show ?thesis
         by (simp add: algebra_simps)
     qed
-    have coeff_in: "?c * len_proof (rule_proof_fun_F rule) \<in> ?S"
+    have coeff_in: "?c * len_proof (rule_proof_fun rule) \<in> ?S"
       using r_in by simp
-    have coeff_le: "?c * len_proof (rule_proof_fun_F rule) \<le> Max ?S"
+    have coeff_le: "?c * len_proof (rule_proof_fun rule) \<le> Max ?S"
       using Max_ge[OF fin_S coeff_in] by simp
-    have mono: "(?c * len_proof (rule_proof_fun_F rule)) * len_proof pr \<le> Max ?S * len_proof pr"
+    have mono: "(?c * len_proof (rule_proof_fun rule)) * len_proof pr \<le> Max ?S * len_proof pr"
       using coeff_le by (simp add: mult_right_mono)
-    have "len_proof (step_F rule sub) \<le> Max ?S * len_proof pr"
+    have "len_proof (step_proof rule sub) \<le> Max ?S * len_proof pr"
       using step_bound' mono by linarith
-    then show "len_proof (step_F rule sub) \<le> poly ?g (len_proof pr)"
+    then show "len_proof (step_proof rule sub) \<le> poly ?g (len_proof pr)"
       by (simp add: algebra_simps)
   qed
 qed
 
-lemma sim_left_step_bound:
+
+lemma sim_step_bound:
   shows "\<exists> bound. \<forall>pr i acc. i \<ge> 0 \<and> i < length (steps pr) \<and> valid_proof F pr \<and> assumptions pr = {} \<longrightarrow>
-            len_proof (sim_left_step pr i acc) \<le> poly bound (len_proof pr) + len_proof acc"
+            len_proof (sim_step pr i acc) \<le> poly bound (len_proof pr) + len_proof acc"
 proof -
   obtain g :: "nat poly" where g_prop:
     "\<forall>rule\<in>rules F. \<forall>pr i sub.
       derived_with i pr rule sub \<and> rule_restricted_sub rule sub \<and> valid_proof F pr \<longrightarrow>
-      len_proof (step_F rule sub) \<le> poly g (len_proof pr)"
-    using step_F_bound by blast
+      len_proof (step_proof rule sub) \<le> poly g (len_proof pr)"
+    using step_proof_bound by blast
   let ?bound = "[:0, 1:] + g"
   show ?thesis
   proof (rule exI[of _ ?bound], intro allI impI)
@@ -2317,34 +685,35 @@ proof -
       using choose_props by simp
     have rsub: "rule_restricted_sub ?rule ?sub"
       using choose_props by simp
-    have step_b: "len_proof (step_F ?rule ?sub) \<le> poly g (len_proof pr)"
+    have step_b: "len_proof (step_proof ?rule ?sub) \<le> poly g (len_proof pr)"
       using g_prop r_in dwith rsub pr_valid by blast
-    have step_eq: "sim_left_step pr i acc = combine_proofs acc (step_F ?rule ?sub)"
+    have step_eq: "sim_step pr i acc = combine_proofs acc (step_proof ?rule ?sub)"
     proof (cases "choose_rule_sub F i pr")
       case (Pair r s)
       then show ?thesis
-        using step_notin i_lt by (simp add: sim_left_step_def Let_def)
+        using step_notin i_lt by (simp add: sim_step_def Let_def)
     qed
-    have "len_proof (sim_left_step pr i acc) = len_proof acc + len_proof (step_F ?rule ?sub)"
+    have "len_proof (sim_step pr i acc) = len_proof acc + len_proof (step_proof ?rule ?sub)"
       using step_eq by simp
     also have "\<dots> \<le> len_proof acc + poly g (len_proof pr)"
       using step_b by simp
     also have "\<dots> \<le> len_proof acc + poly ?bound (len_proof pr)"
       by simp
-    finally show "len_proof (sim_left_step pr i acc) \<le> poly ?bound (len_proof pr) + len_proof acc"
+    finally show "len_proof (sim_step pr i acc) \<le> poly ?bound (len_proof pr) + len_proof acc"
       by (simp add: add.assoc add.commute add.left_commute)
   qed
 qed
 
-lemma sim_left_bound:
+
+lemma sim_bound:
   assumes "valid_proof F pr \<and> assumptions pr = {}"
-  shows "\<exists> bound. len_proof (sim_left pr (thesis pr)) \<le> poly bound (len_proof pr)"
+  shows "\<exists> bound. len_proof (sim pr (thesis pr)) \<le> poly bound (len_proof pr)"
 proof -
   obtain g :: "nat poly" where g_prop:
     "\<forall>pr i acc. i \<ge> 0 \<and> i < length (steps pr) \<and> valid_proof F pr \<and> assumptions pr = {} \<longrightarrow>
-      len_proof (sim_left_step pr i acc) \<le> poly g (len_proof pr) + len_proof acc"
-    using sim_left_step_bound by blast
-  let ?acc = "\<lambda>k. fold (sim_left_step pr) [0..<k] \<lparr>assumptions = assumptions pr, thesis = thesis pr, steps = []\<rparr>"
+      len_proof (sim_step pr i acc) \<le> poly g (len_proof pr) + len_proof acc"
+    using sim_step_bound by blast
+  let ?acc = "\<lambda>k. fold (sim_step pr) [0..<k] \<lparr>assumptions = assumptions pr, thesis = thesis pr, steps = []\<rparr>"
   have pr_valid: "valid_proof F pr"
     using assms by simp
   have pr_assm: "assumptions pr = {}"
@@ -2396,9 +765,9 @@ proof -
       have ih: "len_proof (?acc k) \<le> k * poly g (len_proof pr)"
         using Suc.IH Suc.prems by simp
       have step_b:
-        "len_proof (sim_left_step pr k (?acc k)) \<le> poly g (len_proof pr) + len_proof (?acc k)"
+        "len_proof (sim_step pr k (?acc k)) \<le> poly g (len_proof pr) + len_proof (?acc k)"
         using g_prop k_lt pr_valid pr_assm by simp
-      have "?acc (Suc k) = sim_left_step pr k (?acc k)"
+      have "?acc (Suc k) = sim_step pr k (?acc k)"
         by simp
       then have "len_proof (?acc (Suc k)) \<le> poly g (len_proof pr) + len_proof (?acc k)"
         using step_b by simp
@@ -2411,8 +780,8 @@ proof -
   qed
   let ?bound = "[:0, 1:] * g"
   have final_fold:
-    "len_proof (sim_left pr (thesis pr)) \<le> length (steps pr) * poly g (len_proof pr)"
-    unfolding sim_left_def using fold_bound by simp
+    "len_proof (sim pr (thesis pr)) \<le> length (steps pr) * poly g (len_proof pr)"
+    unfolding sim_def using fold_bound by simp
   also have "\<dots> \<le> len_proof pr * poly g (len_proof pr)"
     using steps_bound by simp
   also have "\<dots> = poly ?bound (len_proof pr)"
@@ -2421,14 +790,14 @@ proof -
     by (rule exI[of _ ?bound])
 qed
 
-lemma simulation_de_morgan_left:
+lemma simulation_de_morgan:
   shows "simulates F F'"
 proof -
   obtain g :: "nat poly" where g_prop:
     "\<forall>pr i acc. i \<ge> 0 \<and> i < length (steps pr) \<and> valid_proof F pr \<and> assumptions pr = {} \<longrightarrow>
-      len_proof (sim_left_step pr i acc) \<le> poly g (len_proof pr) + len_proof acc"
-    using sim_left_step_bound by blast
-  let ?f = "\<lambda>w \<tau>. sim_left w (thesis w)"
+      len_proof (sim_step pr i acc) \<le> poly g (len_proof pr) + len_proof acc"
+    using sim_step_bound by blast
+  let ?f = "\<lambda>w \<tau>. sim w (thesis w)"
   let ?g = "\<lambda>\<tau>. \<tau>"
   let ?p = "[:0, 1:]"
   let ?q = "[:0, 1:] * g"
@@ -2447,8 +816,8 @@ proof -
       using assm by simp
     have pr_props:
       "valid_proof F' (?f w \<tau>) \<and> thesis (?f w \<tau>) = thesis w \<and> assumptions (?f w \<tau>) = {}"
-      using sim_left_proves[of w "sim_left w (thesis w)"] w_valid w_assm by simp
-    let ?acc = "\<lambda>k. fold (sim_left_step w) [0..<k]
+      using sim_proves[of w "sim w (thesis w)"] w_valid w_assm by simp
+    let ?acc = "\<lambda>k. fold (sim_step w) [0..<k]
       \<lparr>assumptions = assumptions w, thesis = thesis w, steps = []\<rparr>"
     have steps_bound: "length (steps w) \<le> len_proof w"
     proof -
@@ -2497,9 +866,9 @@ proof -
         have ih: "len_proof (?acc k) \<le> k * poly g (len_proof w)"
           using Suc.IH Suc.prems by simp
         have step_b:
-          "len_proof (sim_left_step w k (?acc k)) \<le> poly g (len_proof w) + len_proof (?acc k)"
+          "len_proof (sim_step w k (?acc k)) \<le> poly g (len_proof w) + len_proof (?acc k)"
           using g_prop k_lt w_valid w_assm by simp
-        have "?acc (Suc k) = sim_left_step w k (?acc k)"
+        have "?acc (Suc k) = sim_step w k (?acc k)"
           by simp
         then have "len_proof (?acc (Suc k)) \<le> poly g (len_proof w) + len_proof (?acc k)"
           using step_b by simp
@@ -2513,8 +882,8 @@ proof -
     have global_bound:
       "len_proof (?f w \<tau>) \<le> poly ?q (len_proof w)"
     proof -
-      have "len_proof (sim_left w (thesis w)) \<le> length (steps w) * poly g (len_proof w)"
-        unfolding sim_left_def using fold_bound by simp
+      have "len_proof (sim w (thesis w)) \<le> length (steps w) * poly g (len_proof w)"
+        unfolding sim_def using fold_bound by simp
       also have "\<dots> \<le> len_proof w * poly g (len_proof w)"
         using steps_bound by simp
       also have "\<dots> = poly ?q (len_proof w)"
@@ -2559,6 +928,5 @@ proof -
       using sim_case[of w \<tau>] .
   qed
 qed
-
 end
 end
